Cshmgenproof (#110)
* setup done

* changes

* qualify with Ctypes

* parts of transl_step that don't need lemmas done

* parts of proofs not requiring lemmas done

* listed lemmas

* listed lemmas

* setup done

* changes

* qualify with Ctypes

* parts of transl_step that don't need lemmas done

* parts of proofs not requiring lemmas done

* listed lemmas

* listed lemmas

* Add a few lemmas

* up to an error in declaring a lemma

* added all necessary lemmas and finished some of their proofs

* comments on fixes to problems

* finished some lemmas

* Add semantics and proof sketch

* switch extensions for clight

* switch semantics

* correct semantics now

* const int case

* prove cases float, single, long

* prove cases cast and temp var

* prove skip seq

* prove set

* prove seq case

* prove case ifthenelse

* prove case return none

* prove case return some

* prove case skip call

* prove case label

* prove goto

* WIP: internal function

* Add xtype

* prove internal function case

* WIP: transl_initial_states

* prove initial state

* fix lemma

* prove match_cont_call_cont in Comp_Loops

* prove match_cont_is_call_cont in Comp_Loops

* transl_find_label in Comp_Loops

* prove loops

* prove skip or continue

* prove break loop1

* prove skip loop

* prove break loop2 case

* prove builtin case

* transl_expr defined mutually inductively

* fix transl_expr_correct proof

* scaffold transl_expr_lvalue_correct proof

* prove deref case

* prove addrof case

* prove var local case of transl_expr_lvalue

* prove var global

* prove deref

* Add make_load_correct

* rvalue out of lvalue

* prove var local

* var global

* prove make_store_correct

* prove assign case

* prove field case for trasnl_lvalue

* field union

* prove field union

* start call extension

* match_call_cont

* prove match_cont_is_call_cont

* prove call case

* external function

* prove returnstate

* prove nil and switch

* transl_find_label

* WIP

* prove transl_lbl_stmt_1

* prove switch

* prove skip or break switch case

* prove continue switch case

---------

Co-authored-by: Kalarus <notcad@keemail.me>

casestudies/compcert/Cshmgen.v
@@ -1,32 +1,46 @@
-From NFPOP Require Import Loader.
+(*only  Clight Cshminor*)
+From Rocqet Require Import Loader.
+From Rocqet Require Import LibTactics.
 
-From NFPOP Require Import Coqlib.
-From NFPOP Require Import Errors.
-From NFPOP Require Import Values.
-From NFPOP Require Import AST.
-From NFPOP Require Import Integers. 
-From NFPOP Require Import Floats.
-From NFPOP Require Import Memory.
-From NFPOP Require Import Globalenvs.
-From NFPOP Require Import Smallstep.
-From NFPOP Require Import Events.
-From NFPOP Require Import Maps.
-From NFPOP Require Import Linking.
-Require Import NFPOP.CompCert.lib.Ctypes.
-From NFPOP Require Import Cop.
-From NFPOP Require Import Mon.
+From Rocqet Require Import Coqlib.
+From Rocqet Require Import Errors.
+From Rocqet Require Import Values.
+From Rocqet Require Import AST.
+From Rocqet Require Import Integers. 
+From Rocqet Require Import Floats.
+From Rocqet Require Import Memory.
+From Rocqet Require Import Globalenvs.
+From Rocqet Require Import Smallstep.
+From Rocqet Require Import Events.
+From Rocqet Require Import Maps.
+From Rocqet Require Import Linking.
+Require Import Rocqet.CompCert.lib.Ctypes.
+From Rocqet Require Import Cop.
+From Rocqet Require Import Mon.
 Require Import FSets.
 Require Import FSetAVL.
 Require Import Orders.
 Require Import Mergesort.
 Require Import Ordered.
 Require Import Coq.ZArith.ZArith.
-From NFPOP Require Import Prelude.
-From NFPOP Require Import Op.
+From Rocqet Require Import Prelude.
+From Rocqet Require Import Op.
 
 Local Open Scope string_scope.
 Local Open Scope list_scope.
 Open Scope asm.
+
+(* ------------------------------------------------ *)
+(* ------------ Structure of the File ------------- *)
+(* ------------------------------------------------ *)
+(* -------------- Family Clight ------------------- *)
+(* ------------------------------------------------ *)
+(* --- Family CFam (Base family for Csharpminor) -- *)
+(* ------------------------------------------------ *)
+(* ------------ Family Csharpminor ---------------- *)
+(* ------------------------------------------------ *)
+(* ---- Family Cshmgen (Clight -> Csharpminor) ---- *)
+(* ------------------------------------------------ *)
 
 Trait Base. 
 
@@ -79,7 +93,10 @@ Record function : Type := mkfunction {
   fn_body: self__Clight.stmt
 }.
 FEnd function.
-              
+
+FDefinition var_names : list(ident * type) -> list ident :=
+  fun vars => List.map (@fst ident type) vars.
+
 FDefinition fundef := Ctypes.fundef function.
        
 FDefinition type_of_function : function -> type := fun f => 
@@ -92,11 +109,197 @@ FDefinition type_of_fundef : fundef -> type := fun f =>
   end.
 
 FDefinition program := Ctypes.program function.
+(* ------------------------------------------------ *)
+(*                 Semantics for Clight             *)
+(* ------------------------------------------------ *)
+MetaData genv.
+Record genv := { genv_genv :> Genv.t self__Clight.fundef type; genv_cenv :> composite_env }.
+FEnd genv.
+FDefinition globalenv : program -> genv := fun p => 
+  {| self__Clight.genv_genv := Genv.globalenv p; self__Clight.genv_cenv := p.(prog_comp_env) |}.
 
+
+FDefinition env := PTree.t (block * type).
+FDefinition empty_env: env := (PTree.empty (block * type)).
+FDefinition temp_env := PTree.t val.
+
+MetaData alloc_variables.
+Inductive alloc_variables: self__Clight.genv -> self__Clight.env -> mem ->
+                           list (ident * type) ->
+                           self__Clight.env -> mem -> Prop :=
+| alloc_variables_nil:
+  forall ge e m,
+    alloc_variables ge e m nil e m
+| alloc_variables_cons:
+  forall (ge:genv) e m id ty vars m1 b1 m2 e2,
+    Mem.alloc m 0 (sizeof ge ty) = (m1, b1) ->
+    alloc_variables ge (PTree.set id (b1, ty) e) m1 vars e2 m2 ->
+    alloc_variables ge e m ((id, ty) :: vars) e2 m2.
+FEnd alloc_variables.
+
+MetaData create_undef_temps.
+Fixpoint create_undef_temps (temps: list (ident * type)) : self__Clight.temp_env :=
+  match temps with
+  | nil => PTree.empty val
+  | (id, t) :: temps' => PTree.set id Vundef (create_undef_temps temps')
+  end.
+FEnd create_undef_temps.
+
+MetaData bind_parameters.
+Fixpoint bind_parameter_temps (formals: list (ident * type)) (args: list val)
+                              (le: self__Clight.temp_env) : option self__Clight.temp_env :=
+ match formals, args with
+ | nil, nil => Some le
+ | (id, t) :: xl, v :: vl => bind_parameter_temps xl vl (PTree.set id v le)
+ | _, _ => None
+ end.
+FEnd bind_parameters.
+
+FInductive eval_expr : genv -> env -> temp_env -> mem -> expr -> val -> Prop :=
+| eval_Econst_int: forall ge e le m i ty,
+    eval_expr ge e le m (Econst_int i ty) (Vint i)
+| eval_Econst_float: forall ge e le m f ty,
+    eval_expr ge e le m (Econst_float f ty) (Vfloat f)
+| eval_Econst_single: forall ge e le m f ty,
+    eval_expr ge e le m (Econst_single f ty) (Vsingle f)
+| eval_Econst_long: forall ge e le m i ty,
+    eval_expr ge e le m (Econst_long i ty) (Vlong i)
+| eval_Ecast: forall ge e le m a ty v1 v,
+    eval_expr ge e le m a v1 ->
+    Cop.sem_cast v1 (typeof a) ty m = Some v ->
+    eval_expr ge e le m (Ecast a ty) v
+| eval_Etempvar: forall ge e le m id ty v,
+    PTree.get id le = Some v ->
+    eval_expr ge e le m (Etempvar id ty) v.
+
+FInductive cont: Type :=
+| Kstop: cont
+| Kseq: stmt -> cont -> cont. (* Kseq s2 k = after s1 in s1;s2 *)
+
+FRecursion call_cont about cont motive (fun (c : cont) => cont) by _rect.       
+Case Kstop := Kstop.
+Case Kseq s k := (call_cont k).
+FEnd call_cont.
+            
+FRecursion is_call_cont about cont motive (fun (c : cont) => Prop) by _rect.                   
+Case Kstop := True.
+Case Kseq s k := False.
+FEnd is_call_cont.
+            
+FRecursion find_label about stmt motive (fun (_ : stmt) => label -> cont -> option (stmt * cont)) by _rect. 
+Case Sskip := (fun lbl k => None). 
+Case Sset id e := (fun lbl k => None).
+Case Sseq s1 s2 := 
+  (fun lbl k => 
+    match find_label s1 lbl (Kseq s2 k) with
+    | Some sk => Some sk
+    | None => find_label s2 lbl k
+    end). 
+Case Sifthenelse a s1 s2 := 
+ (fun lbl k => 
+     match find_label s1 lbl k with
+      | Some sk => Some sk
+      | None => find_label s2 lbl k
+      end).
+Case Sreturn a := (fun lbl k => None).
+Case Slabel lbl' s' :=  
+  (fun lbl k =>  if ident_eq lbl lbl' then Some(s', k) else find_label s' lbl k).
+Case Sgoto lbl' :=  (fun lbl k => None).
+FEnd find_label.
+
+MetaData state binds State, Callstate, Returnstate.
+Inductive state: Type :=
+  | State
+      (f: function)
+      (s: stmt)
+      (k: cont)
+      (e: env)
+      (le: temp_env)
+      (m: mem) : state
+  | Callstate
+      (fd: fundef)
+      (args: list val)
+      (k: cont)
+      (m: mem) : state
+  | Returnstate
+      (res: val)
+      (k: cont)
+      (m: mem) : state.
+FEnd state.
+
+FDefinition block_of_binding := fun (ge: genv) (id_b_ty: ident * (block * type)) =>
+  match id_b_ty with (id, (b, ty)) => (b, 0, Ctypes.sizeof (self__Clight.genv_cenv ge) ty) end.
+
+FDefinition blocks_of_env : genv -> env -> list (block * Z * Z)  := fun ge e => 
+  List.map (block_of_binding ge) (PTree.elements e).
+
+(* To be overriden in SimplExpr & Cshmgen *)
+FOpaque Definition function_entry : genv -> function -> list val -> mem -> env -> temp_env -> mem -> Prop := cheat.
+
+FInductive step : genv -> state -> trace -> state -> Prop :=  
+| step_skip_seq: forall ge f s k e le m,
+  step ge (State f Sskip (Kseq s k) e le m)
+    E0 (State f s k e le m)
+| step_set: forall ge f id a k e le m v,
+  eval_expr ge e le m a v ->
+  step ge (State f (Sset id a) k e le m)
+    E0 (State f Sskip k e (PTree.set id v le) m)
+| step_seq: forall ge f s1 s2 k e le m,
+  step ge (State f (Sseq s1 s2) k e le m)
+    E0 (State f s1 (Kseq s2 k) e le m)
+| step_ifthenelse: forall ge f a s1 s2 k e le m v1 b,
+    eval_expr ge e le m a v1 ->
+    Cop.bool_val v1 (typeof a) m = Some b ->
+    step ge (State f (Sifthenelse a s1 s2) k e le m)
+      E0 (State f (if b then s1 else s2) k e le m)      
+| step_return_0: forall ge f k e le m m',
+    Mem.free_list m (blocks_of_env ge e) = Some m' ->
+    step ge (State f (Sreturn None) k e le m)
+      E0 (Returnstate Vundef (call_cont k) m')
+| step_return_1: forall ge f a k e le m v v' m',
+    eval_expr ge e le m a v ->
+    Cop.sem_cast v (typeof a) (self__Clight.fn_return f) m = Some v' ->
+    Mem.free_list m (blocks_of_env ge e) = Some m' ->
+    step ge (State f (Sreturn (Some a)) k e le m)
+      E0 (Returnstate v' (call_cont k) m')      
+| step_skip_call: forall ge f k e le m m',
+    is_call_cont k ->
+    Mem.free_list m (blocks_of_env ge e) = Some m' ->
+    step ge (State f Sskip k e le m)
+      E0 (Returnstate Vundef k m')
+| step_label: forall ge f lbl s k e le m,
+  step ge (State f (Slabel lbl s) k e le m)
+    E0 (State f s k e le m)
+| step_goto: forall ge f lbl k e le m s' k',
+  find_label (self__Clight.fn_body f) lbl (call_cont k) = Some (s', k') ->
+  step ge (self__Clight.State f (Sgoto lbl) k e le m)
+    E0 (State f s' k' e le m)    
+| step_internal_function: forall ge f vargs k m e le m1,
+      function_entry ge f vargs m e le m1 ->
+      step ge (Callstate (Internal f) vargs k m)
+        E0 (State f (self__Clight.fn_body f) k e le m1).
+
+MetaData initial_state.
+Inductive initial_state (p: program): state -> Prop :=
+  | initial_state_intro: forall b f m0,
+      let ge := Genv.globalenv p in
+      Genv.init_mem p = Some m0 ->
+      Genv.find_symbol ge p.(prog_main) = Some b ->
+      Genv.find_funct_ptr ge b = Some f ->
+      self__Clight.type_of_fundef f = Tfunction nil type_int32s cc_default ->
+      initial_state p (Callstate f nil self__Clight.Kstop m0).
+FEnd initial_state.
+
+MetaData final_state.
+Inductive final_state: self__Clight.state -> int -> Prop :=
+  | final_state_intro: forall r m,
+      final_state (self__Clight.Returnstate (Vint r) self__Clight.Kstop m) r.
+FEnd final_state.
 FEnd Clight.
 
-
+(* ------------------------------------------------ *)
 (* C family languages: Csharpminor, Cminor, CminorSel *)
+(* ------------------------------------------------ *)
 Family Cfam.
 
 FInductive expr : Type :=
@@ -125,10 +328,187 @@ FDefinition funsig := fun (fd: fundef) =>
   | AST.Internal f => function_sig f
   | AST.External ef => ef_sig ef
   end.
+(* ------------------------------------------------ *)
+(*              Semantics for Cfam                  *)
+(* ------------------------------------------------ *)
+FDefinition genv := Genv.t fundef unit.
+       
+(* Function env/stack space *)
+FOpaque Definition fenv : Type := cheat.
+FOpaque Definition empty_fenv : fenv := cheat.
+       
+FDefinition env := PTree.t val.            
+FDefinition empty_env : env := PTree.empty val.
+       
+MetaData set_params.
+Fixpoint set_params (vl: list val) (il: list ident) {struct il} : self__Cfam.env :=
+ match il, vl with
+ | i1 :: is, v1 :: vs => PTree.set i1 v1 (set_params vs is)
+ | i1 :: is, nil => PTree.set i1 Vundef (set_params nil is)
+ | _, _ => PTree.empty val
+ end.
+FEnd set_params.
+
+MetaData set_locals.
+Fixpoint set_locals (il: list ident) (e: self__Cfam.env) {struct il} : self__Cfam.env :=
+  match il with
+  | nil => e
+  | i1 :: is => PTree.set i1 Vundef (set_locals is e)
+  end.
+FEnd set_locals.
+       
+FDefinition init_env : function -> list val -> env := fun f vargs => 
+  set_locals (function_locals f) (set_params vargs (function_params f)).            
+
+(* Semantics for allocation of variables and binding of parameters at function entry. *)
+FOpaque Definition free_fenv : mem -> fenv -> function -> option mem := cheat.            
+FOpaque Definition alloc_fenv : fenv -> mem -> function -> fenv -> mem -> Prop := cheat.
+       
+MetaData create_undef_temps.
+Fixpoint create_undef_temps (temps: list ident) : self__Cfam.env :=
+ match temps with
+ | nil => PTree.empty val
+ | id :: temps' => PTree.set id Vundef (create_undef_temps temps')
+end.
+FEnd create_undef_temps.
+
+MetaData bind_parameters.
+Fixpoint bind_parameters (formals: list ident) (args: list val)
+             (le: self__Cfam.env) : option self__Cfam.env :=
+ match formals, args with
+ | nil, nil => Some le
+ | id :: xl, v :: vl => bind_parameters xl vl (PTree.set id v le)
+ | _, _ => None
+ end.
+FEnd bind_parameters.
+            
+FInductive cont: Type :=
+| Kstop: cont
+| Kseq: stmt -> cont -> cont.
+                   
+MetaData state binds State, Callstate, Returnstate.
+Inductive state: Type :=
+  | State:(* Execution within a function *)
+      forall (f: function)(* currently executing function *)
+             (s: stmt)(* statement under consideration *)
+             (k:  cont)(* its continuation -- what to do next *)
+             (sp: fenv) (* current "function" environment: i.e stackspace, ... *)
+             (e: self__Cfam.env)(* current local environment *)
+             (m: mem),(* current memory state *)
+      state
+  | Callstate:(* Invocation of a function *)
+      forall (f: fundef)(* function to invoke *)
+             (args: list val)(* arguments provided by caller *)
+             (k: cont)(* what to do next *)
+             (m: mem),(* memory state *)
+      state
+  | Returnstate:(* Return from a function *)
+      forall (v: val)(* Return value *)
+             (k: cont)(* what to do next *)
+             (m: mem),(* memory state *)
+      state.
+FEnd state.
+            
+FRecursion call_cont about cont motive (fun (_ : cont) => cont) by _rect.
+Case Kstop := Kstop.
+Case Kseq s c := (call_cont c).             
+FEnd call_cont.
+               
+FRecursion is_call_cont about cont motive (fun (_ : cont) => Prop) by _rect.
+Case Kstop := True.                   
+Case Kseq s c := False.
+FEnd is_call_cont.              
+
+FDefinition letenv := list val.
+               
+FInductive eval_expr :  genv -> fenv -> env -> mem -> letenv -> expr -> val -> Prop :=
+| eval_Evar: forall ge lenv e le m id v,
+    PTree.get id le = Some v ->
+    eval_expr ge e le m lenv (Evar id) v.
+
+FRecursion find_label about stmt motive (fun (_ : stmt) => label -> cont -> option (stmt * cont)) by _rect.
+Case Sseq s1 s2 := 
+  (fun lbl k => 
+    match find_label s1 lbl (Kseq s2 k) with
+    | Some sk => Some sk
+    | None => find_label s2 lbl k
+    end).
+Case Slabel lbl' s' :=  
+  (fun lbl k =>  if ident_eq lbl lbl' then Some(s', k) else find_label s' lbl k).
+Case _ := (fun lbl k => None).
+FEnd find_label.
+
+(* 
+with find_label_ls (lbl: label) (sl: lbl_stmt) (k: cont)
+                   {struct sl}: option (stmt * cont) :=
+  match sl with
+  | LSnil => None
+  | LScons _ s sl' =>
+      match find_label lbl s (Kseq (seq_of_lbl_stmt sl') k) with
+      | Some sk => Some sk
+      | None => find_label_ls lbl sl' k
+      end
+  end. *)
+
+FInductive step : genv -> state -> trace -> state -> Prop :=
+| step_skip_seq: forall ge f s k e le m,
+    step ge (State f Sskip (Kseq s k) e le m)
+      E0 (State f s k e le m)              
+| step_skip_call: forall ge f k e le m m',
+    is_call_cont k ->                       
+    free_fenv m e f = Some m' ->
+    step ge (State f Sskip k e le m)
+      E0 (Returnstate Vundef k m')
+| step_assign: forall lenv ge f id a k e le m v,
+    eval_expr ge e le m lenv a v ->
+    step ge (State f (Sassign id a) k e le m)
+      E0 (State f Sskip k e (PTree.set id v le) m)
+| step_seq: forall ge f s1 s2 k e le m,
+    step ge (State f (Sseq s1 s2) k e le m)
+      E0 (State f s1 (Kseq s2 k) e le m)              
+| step_return_0: forall ge f k e le m m',                       
+    free_fenv m e f = Some m' ->
+    step ge (State f (Sreturn None) k e le m)
+      E0 (Returnstate Vundef (call_cont k) m')    
+| step_return_1: forall lenv ge f a k e le m v m',
+    eval_expr ge e le m lenv a v ->
+    free_fenv m e f = Some m' ->
+    step ge (State f (Sreturn (Some a)) k e le m)
+      E0 (Returnstate v (call_cont k) m')
+(*| step_internal_function: forall ge f vargs k m m1 e le,          
+    alloc_fenv empty_fenv m f e m1 ->
+    init_env f vargs = le ->                        
+     step ge (Callstate (AST.Internal f) vargs k m)
+       E0 (State f (function_body f) k e le m1)*)
+| step_label: forall ge f lbl s k e le m,
+      step ge (State f (Slabel lbl s) k e le m)
+        E0 (State f s k e le m)
+| step_goto: forall ge f lbl k e le m s' k',
+      find_label (function_body f) lbl (call_cont k) = Some(s', k') ->
+      step ge (State f (Sgoto lbl) k e le m)
+        E0 (State f s' k' e le m).
+            
+MetaData initial_state.
+Inductive initial_state (p: program): state -> Prop :=
+| initial_state_intro: forall b f m0,
+    let ge := Genv.globalenv p in
+    Genv.init_mem p = Some m0 ->
+    Genv.find_symbol ge p.(AST.prog_main) = Some b ->
+    Genv.find_funct_ptr ge b = Some f ->
+    self__Cfam.funsig f = signature_main ->               
+    initial_state p (Callstate f nil Kstop m0).
+FEnd initial_state.
+            
+MetaData final_state.
+Inductive final_state: state -> int -> Prop :=
+| final_state_intro: forall r m,
+   final_state (Returnstate (Vint r) Kstop m) r.
+FEnd final_state.
 
 FEnd Cfam.
-
-(* constants *)
+(* ------------------------------------------------ *)
+(*                 constants                        *)
+(* ------------------------------------------------ *)
 Inductive unary_operation : Type :=
   | Ocast8unsigned: unary_operation(* 8-bit zero extension *)
   | Ocast8signed: unary_operation(* 8-bit sign extension *)
@@ -206,6 +586,10 @@ Inductive binary_operation : Type :=
   | Ocmpl: comparison -> binary_operation(* long signed comparison *)
   | Ocmplu: comparison -> binary_operation. (* long unsigned comparison *)
 
+(* ------------------------------------------------ *)
+(*                      Csharpminor                 *)
+(* ------------------------------------------------ *)
+
 Family Csharpminor extends Cfam.
 FInductive constant : Type :=
 | Ointconst: int -> constant (* integer constant *)
@@ -219,10 +603,10 @@ FInductive expr : Type :=
 | Ebinop : binary_operation -> expr -> expr -> expr. (* binary operation *)                                    
                                                                               
 FInductive stmt : Type :=
-| Sifthenelse: expr -> stmt -> stmt -> stmt
-with lbl_stmts : Type :=
+| Sifthenelse: expr -> stmt -> stmt -> stmt.
+(*with lbl_stmts : Type :=
   | LSnil: lbl_stmts
-  | LScons: option Z -> stmt -> lbl_stmts -> lbl_stmts.
+  | LScons: option Z -> stmt -> lbl_stmts -> lbl_stmts.*)
        
 (* function *)
 MetaData fn.
@@ -239,13 +623,193 @@ FOverride Definition function_body := self__Csharpminor.fn_body.
 FOverride Definition function_locals := self__Csharpminor.fn_temps.
 FOverride Definition function_params := self__Csharpminor.fn_params.
 FOverride Definition function_sig := self__Csharpminor.fn_sig.
+(* ------------------------------------------------ *)
+(*             Semantics for Csharpminor            *)
+(* ------------------------------------------------ *)
+(* function stack environment *)       
+FOverride Definition fenv := PTree.t (block * Z).
+FOverride Definition empty_fenv := PTree.empty (block * Z).
 
+FDefinition block_of_binding := fun (id_b_sz: ident * (block * Z)) => 
+ match id_b_sz with (id, (b, sz)) => (b, 0, sz) end.
+
+FDefinition blocks_of_env : fenv -> list (block * Z * Z) := fun e => 
+  List.map block_of_binding (PTree.elements e).
+
+FOverride Definition free_fenv := fun m e f => Mem.free_list m (blocks_of_env e).
+   
+MetaData alloc_variables.
+Inductive alloc_variables: self__Csharpminor.fenv -> mem ->
+               list (ident * Z) ->
+               self__Csharpminor.fenv -> mem -> Prop :=
+| alloc_variables_nil:
+  forall e m,
+    alloc_variables e m nil e m
+| alloc_variables_cons:
+  forall e m id sz vars m1 b1 m2 e2,
+    Mem.alloc m 0 sz = (m1, b1) ->
+    alloc_variables (PTree.set id (b1, sz) e) m1 vars e2 m2 ->
+    alloc_variables e m ((id, sz) :: vars) e2 m2.
+FEnd alloc_variables.
+         
+FOverride Definition alloc_fenv := fun e m f e' m' => 
+  list_norepet (map fst f.(self__Csharpminor.fn_vars)) /\
+  list_norepet f.(self__Csharpminor.fn_params) /\
+  list_disjoint f.(self__Csharpminor.fn_params) f.(self__Csharpminor.fn_temps) /\
+  alloc_variables self__Csharpminor.empty_fenv m (self__Csharpminor.fn_vars f) e m'.
+
+FRecursion eval_constant about constant motive (fun (_ : constant) => option val) by _rect.
+Case Ointconst := (fun n => Some (Vint n)). 
+Case Ofloatconst := (fun n => Some (Vfloat n)).
+Case Osingleconst := (fun n => Some (Vsingle n)).
+Case Olongconst := (fun n => Some (Vlong n)).
+FEnd eval_constant.
+
+Definition eval_unop (op: unary_operation) (arg: val) : option val :=
+  match op with
+  | Ocast8unsigned => Some (Val.zero_ext 8 arg)
+  | Ocast8signed => Some (Val.sign_ext 8 arg)
+  | Ocast16unsigned => Some (Val.zero_ext 16 arg)
+  | Ocast16signed => Some (Val.sign_ext 16 arg)
+  | Onegint => Some (Val.negint arg)
+  | Onotint => Some (Val.notint arg)
+  | Onegf => Some (Val.negf arg)
+  | Oabsf => Some (Val.absf arg)
+  | Onegfs => Some (Val.negfs arg)
+  | Oabsfs => Some (Val.absfs arg)
+  | Osingleoffloat => Some (Val.singleoffloat arg)
+  | Ofloatofsingle => Some (Val.floatofsingle arg)
+  | Ointoffloat => Val.intoffloat arg
+  | Ointuoffloat => Val.intuoffloat arg
+  | Ofloatofint => Val.floatofint arg
+  | Ofloatofintu => Val.floatofintu arg
+  | Ointofsingle => Val.intofsingle arg
+  | Ointuofsingle => Val.intuofsingle arg
+  | Osingleofint => Val.singleofint arg
+  | Osingleofintu => Val.singleofintu arg
+  | Onegl => Some (Val.negl arg)
+  | Onotl => Some (Val.notl arg)
+  | Ointoflong => Some (Val.loword arg)
+  | Olongofint => Some (Val.longofint arg)
+  | Olongofintu => Some (Val.longofintu arg)
+  | Olongoffloat => Val.longoffloat arg
+  | Olonguoffloat => Val.longuoffloat arg
+  | Ofloatoflong => Val.floatoflong arg
+  | Ofloatoflongu => Val.floatoflongu arg
+  | Olongofsingle => Val.longofsingle arg
+  | Olonguofsingle => Val.longuofsingle arg
+  | Osingleoflong => Val.singleoflong arg
+  | Osingleoflongu => Val.singleoflongu arg
+  end.
+
+Definition eval_binop
+            (op: binary_operation) (arg1 arg2: val) (m: mem): option val :=
+  match op with
+  | Oadd => Some (Val.add arg1 arg2)
+  | Osub => Some (Val.sub arg1 arg2)
+  | Omul => Some (Val.mul arg1 arg2)
+  | Odiv => Val.divs arg1 arg2
+  | Odivu => Val.divu arg1 arg2
+  | Omod => Val.mods arg1 arg2
+  | Omodu => Val.modu arg1 arg2
+  | Oand => Some (Val.and arg1 arg2)
+  | Oor => Some (Val.or arg1 arg2)
+  | Oxor => Some (Val.xor arg1 arg2)
+  | Oshl => Some (Val.shl arg1 arg2)
+  | Oshr => Some (Val.shr arg1 arg2)
+  | Oshru => Some (Val.shru arg1 arg2)
+  | Oaddf => Some (Val.addf arg1 arg2)
+  | Osubf => Some (Val.subf arg1 arg2)
+  | Omulf => Some (Val.mulf arg1 arg2)
+  | Odivf => Some (Val.divf arg1 arg2)
+  | Oaddfs => Some (Val.addfs arg1 arg2)
+  | Osubfs => Some (Val.subfs arg1 arg2)
+  | Omulfs => Some (Val.mulfs arg1 arg2)
+  | Odivfs => Some (Val.divfs arg1 arg2)
+  | Oaddl => Some (Val.addl arg1 arg2)
+  | Osubl => Some (Val.subl arg1 arg2)
+  | Omull => Some (Val.mull arg1 arg2)
+  | Odivl => Val.divls arg1 arg2
+  | Odivlu => Val.divlu arg1 arg2
+  | Omodl => Val.modls arg1 arg2
+  | Omodlu => Val.modlu arg1 arg2
+  | Oandl => Some (Val.andl arg1 arg2)
+  | Oorl => Some (Val.orl arg1 arg2)
+  | Oxorl => Some (Val.xorl arg1 arg2)
+  | Oshll => Some (Val.shll arg1 arg2)
+  | Oshrl => Some (Val.shrl arg1 arg2)
+  | Oshrlu => Some (Val.shrlu arg1 arg2)
+  | Ocmp c => Some (Val.cmp c arg1 arg2)
+  | Ocmpu c => Some (Val.cmpu (Mem.valid_pointer m) c arg1 arg2)
+  | Ocmpf c => Some (Val.cmpf c arg1 arg2)
+  | Ocmpfs c => Some (Val.cmpfs c arg1 arg2)
+  | Ocmpl c => Val.cmpl c arg1 arg2
+  | Ocmplu c => Val.cmplu (Mem.valid_pointer m) c arg1 arg2
+  end.
+
+FInductive eval_expr :  genv -> fenv -> env -> mem -> letenv -> expr -> val -> Prop :=
+  | eval_Econst: forall ge lenv e le m cst v,
+      eval_constant cst = Some v ->
+      eval_expr ge e le m lenv (Econst cst) v
+  | eval_Eunop: forall ge lenv e le m op a1 v1 v,
+      eval_expr ge e le m lenv a1 v1 ->
+      eval_unop op v1 = Some v ->
+      eval_expr ge e le m lenv (Eunop op a1) v
+  | eval_Ebinop: forall ge lenv e le m op a1 a2 v1 v2 v,
+      eval_expr ge e le m lenv a1 v1 ->
+      eval_expr ge e le m lenv a2 v2 ->
+      eval_binop op v1 v2 m = Some v ->
+      eval_expr ge e le m lenv (Ebinop op a1 a2) v.
+
+FRecursion find_label.
+Case Sifthenelse a s1 s2 := 
+(fun lbl k => 
+   match find_label s1 lbl k with
+   | Some sk => Some sk
+   | None => find_label s2 lbl k
+   end).
+FEnd find_label.
+
+FInductive step : genv -> state -> trace -> state -> Prop :=
+| step_ifthenelse: forall lenv ge f a s1 s2 k sp e m v b,
+    eval_expr ge sp e m lenv a v ->
+    Val.bool_of_val v b ->
+    step ge (self__Csharpminor.State f (Sifthenelse a s1 s2) k sp e m)
+      E0 (self__Csharpminor.State f (if b then s1 else s2) k sp e m)
+| step_label: forall ge f lbl s k e le m,
+    step ge (self__Csharpminor.State f (Slabel lbl s) k e le m)
+      E0 (self__Csharpminor.State f s k e le m)
+| step_internal_function: forall ge f vargs k m m1 e le,
+   Val.has_argtype_list vargs (self__Csharpminor.fn_sig f).(sig_args) ->
+   list_norepet (map fst (self__Csharpminor.fn_vars f)) ->
+   list_norepet (self__Csharpminor.fn_params f) ->
+   list_disjoint (self__Csharpminor.fn_params f) (self__Csharpminor.fn_temps f) ->
+   alloc_variables empty_fenv m (self__Csharpminor.fn_vars f) e m1 ->
+   bind_parameters (self__Csharpminor.fn_params f) vargs (create_undef_temps (self__Csharpminor.fn_temps f)) = Some le ->
+   step ge (Callstate (AST.Internal f) vargs k m)
+     E0 (State f (self__Csharpminor.fn_body f) k e le m1).      
 FEnd Csharpminor.
 
-
-(* Clight -> Csharpminor *)
+(* ------------------------------------------------ *)
+(*             Cshmgen (Clight -> Csharpminor)      *)
+(* ------------------------------------------------ *)
 Family Cshmgen.
-Family S extends Clight. FEnd S.
+Family S extends Clight.
+
+Inherit find_label.
+
+MetaData function_entry2.
+Inductive function_entry2 (ge: genv) (f: function) (vargs: list val) (m: mem) (e: env) (le: temp_env) (m': mem) : Prop :=
+  | function_entry2_intro:
+      list_norepet (var_names f.(fn_vars)) ->
+      list_norepet (var_names f.(fn_params)) ->
+      list_disjoint (var_names f.(fn_params)) (var_names f.(fn_temps)) ->
+      alloc_variables ge empty_env m f.(fn_vars) e m' ->
+      bind_parameter_temps f.(fn_params) vargs (create_undef_temps f.(fn_temps)) = Some le ->
+      function_entry2 ge f vargs m e le m'.
+FEnd function_entry2.
+FOverride Definition function_entry := function_entry2.
+FEnd S.
 Family T extends Csharpminor. FEnd T.
 
 FDefinition make_intconst := fun (n: int) => T.Econst (T.Ointconst n).
@@ -602,28 +1166,32 @@ FDefinition transl_binop
   | Cop.Oge => make_cmp Cge a ta b tb
   end.
 
-FRecursion transl_expr about S.expr motive (fun (_ : S.expr) => composite_env -> res T.expr) by _rect.
-Case Econst_int n ty := (fun ce => OK(make_intconst n)). 
-Case Econst_float n ty := (fun ce => OK(make_floatconst n)).
-Case Econst_single n ty := (fun ce => OK(make_singleconst n)).
-Case Econst_long n ty := (fun ce => OK(make_longconst n)).
-Case Etempvar id ty := (fun ce => OK(T.Evar id)). 
-Case Esizeof ty' ty := (fun ce => do sz <- sizeof ce ty'; OK(make_ptrofsconst sz)).
-Case Ealignof ty' ty := (fun ce => do al <- alignof ce ty'; OK(make_ptrofsconst al)).
-Case Ecast b ty := (fun ce => do tb <- transl_expr b ce; make_cast (S.typeof b) ty tb).
+FRecursion translate_expression about S.expr motive
+   (fun (_ : S.expr) => composite_env -> res T.expr * res (T.expr * bitfield)) by _rect.
+Case Econst_int n ty := (fun ce => (OK(make_intconst n),  Error(msg "Cshmgen.transl_lvalue"))). 
+Case Econst_float n ty := (fun ce => (OK(make_floatconst n), Error(msg "Cshmgen.transl_lvalue"))).
+Case Econst_single n ty := (fun ce => (OK(make_singleconst n), Error(msg "Cshmgen.transl_lvalue"))).
+Case Econst_long n ty := (fun ce => (OK(make_longconst n), Error(msg "Cshmgen.transl_lvalue"))).
+Case Etempvar id ty := (fun ce => (OK(T.Evar id), Error(msg "Cshmgen.transl_lvalue"))). 
+Case Esizeof ty' ty := (fun ce => (do sz <- sizeof ce ty'; OK(make_ptrofsconst sz), Error(msg "Cshmgen.transl_lvalue"))).
+Case Ealignof ty' ty := (fun ce => (do al <- alignof ce ty'; OK(make_ptrofsconst al), Error(msg "Cshmgen.transl_lvalue"))).
+Case Ecast b ty := (fun ce => (do tb <- fst (translate_expression b ce); make_cast (S.typeof b) ty tb, Error(msg "Cshmgen.transl_lvalue"))).
 Case Eunop op b ty :=
 (fun ce =>
-   do tb <- transl_expr b ce;
-    transl_unop op tb (S.typeof b)).
+   (do tb <- fst (translate_expression b ce);
+       transl_unop op tb (S.typeof b),
+      Error(msg "Cshmgen.transl_lvalue"))).
 Case Ebinop op b c ty :=
 (fun ce =>
-   do tb <- transl_expr b ce;
-   do tc <- transl_expr c ce;
-   transl_binop ce op tb (S.typeof b) tc (S.typeof c)).
-FEnd transl_expr.
+   (do tb <- fst (translate_expression b ce);
+   do tc <- fst (translate_expression c ce);
+   transl_binop ce op tb (S.typeof b) tc (S.typeof c),
+   Error(msg "Cshmgen.transl_lvalue"))).
+FEnd translate_expression.
+
+FDefinition transl_expr := fun e ce => fst (translate_expression e ce).
       
-FRecursion transl_stmt about S.stmt motive (fun (_ : S.stmt) => composite_env -> type -> nat -> nat -> res T.stmt)
-     with transl_lbl_stmt about T.lbl_stmts motive (fun (_: S.lbl_stmts) => composite_env -> type -> nat -> nat -> res T.lbl_stmts) by _rect.
+FRecursion transl_stmt about S.stmt motive (fun (_ : S.stmt) => composite_env -> type -> nat -> nat -> res T.stmt) by _rect.     
 Case Sskip := (fun ce tyret nbrk ncnt => OK T.Sskip).   
 Case Sset x b :=
 (fun ce tyret nbrk ncnt => 
@@ -654,21 +1222,14 @@ Case Slabel lbl s :=
   do ts <- transl_stmt s ce tyret nbrk ncnt;
   OK (T.Slabel lbl ts)).
 Case Sgoto lbl := (fun ce tyret nbrk ncnt => OK (T.Sgoto lbl)).
-
-Case LSnil := (fun ce tyret nbrk ncnt => OK T.LSnil).
-Case LScons n s sl' :=
-  (fun ce tyret nbrk ncnt =>
-      do ts <- transl_stmt s ce tyret nbrk ncnt;
-      do tsl' <- transl_lbl_stmt sl' ce tyret nbrk ncnt;
-      OK (T.LScons n ts tsl')).
-FEnd transl_stmt with transl_lbl_stmt.
+FEnd transl_stmt.
 
 (* Translation of functions *)
 FDefinition transl_var := fun (ce: composite_env) (v: ident * type) =>
   do sz <- sizeof ce (snd v); OK (fst v, sz).
       
 FDefinition signature_of_function := fun (f: S.function) =>
-  {| sig_args := map typ_of_type (map snd (S.fn_params f));
+  {| sig_args := map argtype_of_type (map snd (S.fn_params f));
     sig_res  := rettype_of_type (S.fn_return f);
     sig_cc   := S.fn_callconv f |}.
       
@@ -698,6 +1259,790 @@ FDefinition transl_globvar := fun (id: ident) (ty: type) => OK tt.
 
 FDefinition transl_program : S.program -> res T.program := fun p => 
   transform_partial_program2 (transl_fundef p.(prog_comp_env)) transl_globvar p.
+(* ------------------------------------------------ *)
+(* ---------------- Cshmgenproof ------------------ *)
+(* ------------------------------------------------ *)
+
+
+MetaData match_fundef.
+Inductive match_fundef (p: self__Cshmgen.S.program) : self__Cshmgen.S.fundef -> self__Cshmgen.T.fundef -> Prop :=
+  | match_fundef_internal: forall f tf,
+      self__Cshmgen.transl_function p.(prog_comp_env) f = OK tf ->
+      match_fundef p (Ctypes.Internal f) (AST.Internal tf)
+  | match_fundef_external: forall ef args res cc,
+      ef_sig ef = signature_of_type args res cc ->
+      match_fundef p (Ctypes.External ef args res cc) (AST.External ef).
+FEnd match_fundef.
+
+FDefinition match_varinfo : type -> unit -> Prop := fun v tv => True.
+
+FDefinition match_prog : S.program -> T.program -> Prop := fun p tp =>
+  match_program_gen match_fundef match_varinfo p p tp.
+
+FLemma transl_sizeof:
+  forall (cunit prog: S.program) t sz,
+  linkorder cunit prog ->
+  sizeof cunit.(prog_comp_env) t = OK sz ->
+  sz = Ctypes.sizeof prog.(prog_comp_env) t.
+FProofLemma.
+  intros. destruct H.
+  unfold sizeof in H0. destruct (complete_type (prog_comp_env cunit) t) eqn:C; inv H0.
+  symmetry. apply Ctypes.sizeof_stable; auto.
+Qed. CloseFLemma.
+
+(*
+Variable prog: Clight.program.
+Variable tprog: Csharpminor.program.
+Hypothesis TRANSL: match_prog prog tprog.
+
+Let ge := globalenv prog.
+Let tge := Genv.globalenv tprog.
+ *)
+(* ------------------------------------------------ *)
+(*                  CONSTRUCTORS                    *)
+(* ------------------------------------------------ *)
+FLemma make_intconst_correct:
+  forall lenv ge n e le m,
+  T.eval_expr ge e le m lenv (make_intconst n) (Vint n).
+FProofLemma.
+intros. unfold make_intconst. fconstructor. fsimpl.
+reflexivity.
+Qed. CloseFLemma.
+
+FLemma make_floatconst_correct:
+  forall lenv ge n e le m,
+  T.eval_expr ge e le m lenv (make_floatconst n) (Vfloat n).
+FProofLemma.
+intros. unfold make_floatconst. fconstructor.
+fsimpl. reflexivity.
+Qed. CloseFLemma.
+
+FLemma make_singleconst_correct:
+  forall lenv ge n e le m,
+  T.eval_expr ge e le m lenv (make_singleconst n) (Vsingle n).
+FProofLemma.
+intros. unfold make_singleconst. fconstructor.
+fsimpl. reflexivity.
+Qed. CloseFLemma.
+
+FLemma make_longconst_correct:
+  forall lenv ge n e le m,
+  T.eval_expr ge e le m lenv (make_longconst n) (Vlong n).
+FProofLemma.
+intros. unfold make_floatconst. fconstructor.
+fsimpl. reflexivity.
+Qed. CloseFLemma.
+
+FLemma make_ptrofsconst_correct:
+  forall lenv ge n e le m,
+  T.eval_expr ge e le m lenv (make_ptrofsconst n) (Vptrofs (Ptrofs.repr n)).
+FProofLemma.
+  intros. unfold Vptrofs, make_ptrofsconst. destruct Archi.ptr64 eqn:SF.
+- replace (Ptrofs.to_int64 (Ptrofs.repr n)) with (Int64.repr n).
+  apply make_longconst_correct.
+  symmetry; auto with ptrofs.
+- replace (Ptrofs.to_int (Ptrofs.repr n)) with (Int.repr n).
+  apply make_intconst_correct.
+  symmetry; auto with ptrofs.
+Qed. CloseFLemma.
+
+FLemma make_singleoffloat_correct:
+  forall lenv ge a n e le m,
+  T.eval_expr ge e le m lenv a (Vfloat n) ->
+  T.eval_expr ge e le m lenv (make_singleoffloat a) (Vsingle (Float.to_single n)).
+FProofLemma.
+  intros. fconstructor.
+Qed. CloseFLemma.
+
+FLemma make_floatofsingle_correct:
+  forall lenv ge a n e le m,
+  T.eval_expr ge e le m lenv a (Vsingle n) ->
+  T.eval_expr ge e le m lenv (make_floatofsingle a) (Vfloat (Float.of_single n)).
+FProofLemma.
+  intros. fconstructor.
+Qed. CloseFLemma.
+
+FLemma make_floatofint_correct:
+  forall lenv ge a n sg e le m,
+  T.eval_expr ge e le m lenv a (Vint n) ->
+  T.eval_expr ge e le m lenv (make_floatofint a sg) (Vfloat (cast_int_float sg n)).
+FProofLemma.
+  intros. unfold make_floatofint, cast_int_float.
+  destruct sg; fconstructor; eauto.
+Qed. CloseFLemma.
+
+(* Hint Extern 2 (@eq trace _ _) => traceEq: cshm. *)
+(* helper lemmas for make_cmpu_ne_zero_correct *)
+FLemma default_Vint :
+  forall lenv ge e le m a n,
+    T.eval_expr ge e le m lenv a (Vint n) ->
+    T.eval_expr ge e le m lenv (T.Ebinop (Ocmpu Cne) a (make_intconst Int.zero))
+      (Vint (if Int.eq n Int.zero then Int.zero else Int.one)).
+FProofLemma.
+intros. fconstructor; eauto.
+- fconstructor. fsimpl. reflexivity.
+- simpl. unfold Val.cmpu, Val.cmpu_bool.
+unfold Int.cmpu. destruct (Int.eq n Int.zero); auto.
+Qed. CloseFLemma.
+
+FLemma cmp :
+  forall n ob,
+    Val.of_optbool ob = Vint n ->
+    n = (if Int.eq n Int.zero then Int.zero else Int.one).
+FProofLemma.
+intros. destruct ob; simpl in H; inv H. destruct b; inv H1.
+- rewrite Int.eq_false; auto. apply Int.one_not_zero.
+- rewrite Int.eq_true. auto.
+Qed. CloseFLemma.
+(* inversion lemmas for use in make_cmpu_ne_zero_correct *)
+Closing Fact eval_Ebinop_inv :
+  forall ge lenv e le m op a1 a2 v1 v2 v,
+    T.eval_expr ge e le m lenv (T.Ebinop op a1 a2) v ->
+    T.eval_expr ge e le m lenv a1 v1 /\
+      T.eval_expr ge e le m lenv a2 v2 /\
+      eval_binop op v1 v2 m = Some v
+    by plain {intros until tmp; intros H; inv H; eauto}.
+
+FInduction make_cmpu_ne_zero_correct
+  about T.eval_expr motive
+  fun ge e le m lenv a v (_ : T.eval_expr ge e le m lenv a v) =>
+    forall (* ge e le m lenv a v (_ : T.eval_expr ge e le m lenv a v)*) n,
+      T.eval_expr ge e le m lenv a (Vint n) ->
+      T.eval_expr ge e le m lenv (make_cmpu_ne_zero a)
+        (Vint (if Int.eq n Int.zero then Int.zero else Int.one)).
+FProof.
+all:
+  intros; pose proof default_Vint; pose proof cmp; 
+  fsimpl; auto. apply cheat.
+(*destruct op; fsimpl; eauto.
+all: eapply eval_Ebinop_inv in H1; destruct H1 as [hyp1 [hyp2 hyp3]];
+  fconstructor; eauto; rewrite hyp3; decEq; decEq;
+  simpl in hyp3.
+- inv hyp3; eauto.
+- inv hyp3; eauto.
+- inv hyp3; eauto.
+- inv hyp3; eauto.
+- unfold Val.cmpl in hyp3. destruct (Val.cmpl_bool c ?[v13] ?[v23])
+    as [[]|]; inv hyp3; reflexivity.
+- unfold Val.cmplu in hyp3. destruct (Val.cmplu_bool (Mem.valid_pointer m) c ?[v1] ?[v2])
+    as [[]|]; inv hyp3; reflexivity.*)
+Qed. FEnd make_cmpu_ne_zero_correct.
+
+
+(* For proving make_cmpu_ne_zero_correct_ptr *)
+FLemma default_Vone :
+  forall lenv ge e le m a b i,
+    T.eval_expr ge e le m lenv a (Vptr b i) ->
+    Archi.ptr64 = false ->
+    Mem.weak_valid_pointer m b (Ptrofs.unsigned i) = true ->
+    T.eval_expr ge e le m lenv (T.Ebinop (Ocmpu Cne) a (make_intconst Int.zero)) Vone.
+FProofLemma.
+intros. fconstructor. { fconstructor. fsimpl. reflexivity. }
+simpl. unfold Val.cmpu, Val.cmpu_bool.
+unfold Mem.weak_valid_pointer in H1. rewrite H0, H1.
+rewrite Int.eq_true; auto.
+Qed. CloseFLemma.
+
+FLemma of_optbool :
+  forall ob b i,
+    Some (Val.of_optbool ob) <> Some (Vptr b i).
+FProofLemma.
+intros. destruct ob as [[]|]; discriminate.
+Qed. CloseFLemma.
+FLemma of_bool :
+  forall ob b i,
+    option_map Val.of_bool ob <> Some (Vptr b i).
+FProofLemma.
+intros. destruct ob as [[]|]; discriminate.
+Qed. CloseFLemma.
+
+FInduction make_cmpu_ne_zero_correct_ptr
+  about T.eval_expr motive
+  fun ge e le m lenv a v (_ : T.eval_expr ge e le m lenv a v) =>
+    forall b i,
+  T.eval_expr ge e le m lenv a (Vptr b i) ->
+  Archi.ptr64 = false ->
+  Mem.weak_valid_pointer m b (Ptrofs.unsigned i) = true ->
+  T.eval_expr ge e le m lenv (make_cmpu_ne_zero a) Vone.
+FProof.
+all: intros;
+  pose proof default_Vone;
+  pose proof of_optbool;
+  pose proof of_bool;
+  fsimpl; eauto.
+unfold make_cmpu_ne_zero_helper.
+apply cheat.
+(*destruct op; fsimpl; eauto.
+all: eapply eval_Ebinop_inv in H1; destruct H1 as [hyp1 [hyp2 hyp3]];
+  eelim of_optbool; eauto.
+all: eelim of_bool; eauto.*)
+Qed.  FEnd make_cmpu_ne_zero_correct_ptr.
+
+FLemma make_cast_int_correct:
+  forall lenv ge e le m a n sz si,
+  T.eval_expr ge e le m lenv a (Vint n) ->
+  T.eval_expr ge e le m lenv (make_cast_int a sz si) (Vint (cast_int_int sz si n)).
+FProofLemma.
+intros. unfold make_cast_int, cast_int_int.
+destruct sz; destruct si; eauto;try fconstructor;
+  eapply make_cmpu_ne_zero_correct in H; apply H ; auto.    
+Qed. CloseFLemma.
+
+FLemma make_longofint_correct:
+  forall lenv ge e le m a n si,
+  T.eval_expr ge e le m lenv a (Vint n) ->
+  T.eval_expr ge e le m lenv (make_longofint a si) (Vlong (cast_int_long si n)).
+FProofLemma.
+intros. unfold make_longofint, cast_int_long. destruct si; eauto;fconstructor.
+Qed. CloseFLemma.
+
+Ltac InvEval :=
+  match goal with
+  | [ H: None = Some _ |- _ ] => discriminate
+  | [ H: Some _ = Some _ |- _ ] => inv H; InvEval
+  | [ H: match ?x with Some _ => _ | None => _ end = Some _ |- _ ] => destruct x eqn:?; InvEval
+  | [ H: match ?x with true => _ | false => _ end = Some _ |- _ ] => destruct x eqn:?; InvEval
+  | _ => idtac
+  end.
+FLemma make_cast_correct:
+  forall lenv ge e le m a b v ty1 ty2 v',
+  make_cast ty1 ty2 a = OK b ->
+  T.eval_expr ge e le m lenv a v ->
+  sem_cast v ty1 ty2 m = Some v' ->
+  T.eval_expr ge e le m lenv b v'.
+FProofLemma.
+intros. unfold make_cast, sem_cast in *;
+  destruct (classify_cast ty1 ty2); inv H; destruct v; InvEval; eauto;
+apply cheat.
+(* without cshm database, more cases for manual proof*)
+Qed. CloseFLemma. 
+
+FLemma make_boolean_correct:
+ forall lenv ge e le m a v ty b,
+  T.eval_expr ge e le m lenv a v ->
+  bool_val v ty m = Some b ->
+  exists vb,
+    T.eval_expr ge e le m lenv (make_boolean a ty) vb
+    /\ Val.bool_of_val vb b.
+FProofLemma.
+intros. unfold make_boolean. unfold bool_val in H0.
+  destruct (classify_bool ty); destruct v; InvEval.
+- (* int *)
+  econstructor; split.
+  + eapply make_cmpu_ne_zero_correct ; eauto.
+  + destruct (Int.eq i Int.zero); simpl; constructor.
+- (* ptr 32 bits *)
+  exists Vone; split. eapply make_cmpu_ne_zero_correct_ptr; eauto. constructor.
+- (* long *)
+  econstructor; split.
+  + fconstructor. { fconstructor. fsimpl. reflexivity. }
+    simpl. unfold Val.cmplu. simpl. eauto.
+  + destruct (Int64.eq i Int64.zero); simpl; constructor.
+- (* ptr 64 bits *)
+  exists Vone; split.
+  fconstructor. { fconstructor. fsimpl. reflexivity. }
+  simpl. unfold Val.cmplu, Val.cmplu_bool.
+  unfold Mem.weak_valid_pointer in Heqb0. rewrite Heqb0, Heqb1, Int64.eq_true. reflexivity.
+  constructor.
+- (* float *)
+  econstructor; split. fconstructor. { fconstructor. fsimpl. reflexivity. }
+  simpl. eauto.
+  unfold Val.cmpf, Val.cmpf_bool. simpl. rewrite <- Float.cmp_ne_eq.
+  destruct (Float.cmp Cne f Float.zero); constructor.
+- (* single *)
+  econstructor; split.
+  fconstructor. { fconstructor. fsimpl. reflexivity. } simpl. eauto.
+  unfold Val.cmpfs, Val.cmpfs_bool. simpl. rewrite <- Float32.cmp_ne_eq.
+  destruct (Float32.cmp Cne f Float32.zero); constructor.
+Qed. CloseFLemma.
+
+(* ------------------------------------------------ *)
+(*                  CORRECTNESS                     *)
+(* ------------------------------------------------ *)
+(*FLemma function_ptr_translated:
+  forall ge tge prog tprog v f,
+  Genv.find_funct_ptr ge v = Some f ->
+  exists cu tf, Genv.find_funct_ptr tge v = Some tf /\ match_fundef cu f tf /\ linkorder cu prog.
+  *)
+MetaData match_env.
+
+Record match_env
+  (prog: S.program)
+  (e: S.env) (te: T.fenv) : Prop :=
+ mk_match_env {
+   me_local:
+     forall id b ty,
+       e!id = Some (b, ty) ->
+       let ge := S.globalenv prog in 
+       te!id = Some (b, Ctypes.sizeof (S.genv_cenv ge) ty);
+   me_local_inv:
+     forall id b sz,
+     te!id = Some (b, sz) -> exists ty, e!id = Some(b, ty)
+}.
+FEnd match_env.
+
+FLemma match_env_same_blocks:
+  forall ge prog e te,
+  match_env prog e te ->
+  T.blocks_of_env te = S.blocks_of_env ge e.
+FProofLemma.
+intros.
+set (R := fun (x: (block * type)) (y: (block * Z)) =>
+            match x, y with
+            | (b1, ty), (b2, sz) => b2 = b1 /\ sz = Ctypes.sizeof (S.genv_cenv ge) ty
+            end).
+assert (list_forall2
+          (fun i_x i_y => fst i_x = fst i_y /\ R (snd i_x) (snd i_y))
+          (PTree.elements e) (PTree.elements te)).
+{ apply PTree.elements_canonical_order. 
+  - intros id [b ty] GET.
+    exists (b, Ctypes.sizeof (S.genv_cenv ge) ty); split.
+    (* type needed different for ge 
+    exists (b, Ctypes.sizeof (S.genv_cenv (S.globalenv ge)) ty); split.*)
+    + destruct ge. (*eapply me_local; eauto.*) apply cheat.
+    + red; auto.
+  - intros id [b sz] GET. exploit me_local_inv; eauto. intros [ty EQ].
+    exploit me_local; eauto. intros EQ1.
+    exists (b, ty); split; eauto.
+    red; split.
+    + congruence.
+    (* ge in EQ1 is the standard ge, but in environment outside is not*) 
+    + apply cheat. }
+unfold T.blocks_of_env, S.blocks_of_env.
+generalize H0. induction 1. auto.
+simpl. f_equal; auto.
+unfold T.block_of_binding, S.block_of_binding.
+destruct a1 as [id1 [blk1 ty1]]. destruct b1 as [id2 [blk2 sz2]].
+simpl in *. destruct H1 as [A [B C]]. congruence.
+Qed. CloseFLemma.
+
+FLemma match_env_free_blocks:
+  forall ge prog e te m m',
+  match_env prog e te ->
+  Mem.free_list m (S.blocks_of_env ge e) = Some m' ->
+  Mem.free_list m (T.blocks_of_env te) = Some m'.
+FProofLemma.
+intros. rewrite (match_env_same_blocks ge prog _ _ H). auto.
+Qed. CloseFLemma.
+
+FLemma match_env_empty:
+  forall prog,
+  match_env prog S.empty_env T.empty_fenv.
+FProofLemma.
+  unfold S.empty_env, T.empty_fenv.
+  constructor.
+  intros until ty. repeat rewrite PTree.gempty. congruence.
+  intros until sz. rewrite PTree.gempty. congruence.
+Qed. CloseFLemma.  
+
+FLemma match_env_alloc_variables:
+  forall prog cunit, linkorder cunit prog ->
+  forall ge e1 m1 vars e2 m2, S.alloc_variables ge e1 m1 vars e2 m2 ->
+  forall tvars te1,
+  mmap (transl_var cunit.(prog_comp_env)) vars = OK tvars ->
+  match_env prog e1 te1 ->
+  exists te2,
+  T.alloc_variables te1 m1 tvars te2 m2
+  /\ match_env prog e2 te2.
+FProofLemma.
+(* induction 2; simpl; intros.
+- inv H0. exists te1; split. constructor. auto.
+- monadInv H2. monadInv EQ. simpl in *.
+  exploit transl_sizeof. eexact H. eauto. intros SZ; rewrite SZ.
+  exploit (IHalloc_variables x0 (PTree.set id (b1, Ctypes.sizeof (S.genv_cenv ge) ty) te1)).
+  + auto.
+  + constructor.
+    * (* me_local *)
+      intros until ty0. repeat rewrite PTree.gsspec.
+      destruct (peq id0 id); intros.
+      -- (*constructor creates a ge0 variable, compcert didn't have this behaviour*)
+        apply cheat.
+      -- eapply me_local; eauto.
+    * (* me_local_inv *)
+      intros until sz. repeat rewrite PTree.gsspec.
+      destruct (peq id0 id); intros.
+      -- exists ty; congruence.
+      -- eapply me_local_inv; eauto.
+  + intros [te2 [ALLOC MENV]].
+    exists te2; split;eauto.
+    econstructor; eauto.
+ *)
+apply cheat.
+Qed. CloseFLemma.
+FLemma create_undef_temps_match:
+  forall temps,
+  T.create_undef_temps (map fst temps) = S.create_undef_temps temps.
+FProofLemma.
+induction temps; simpl. auto.
+destruct a as [id ty]. simpl. decEq. auto.
+Qed. CloseFLemma.
+
+FLemma bind_parameter_temps_match:
+  forall vars vals le1 le2,
+  S.bind_parameter_temps vars vals le1 = Some le2 ->
+  T.bind_parameters (map fst vars) vals le1 = Some le2.
+FProofLemma.
+induction vars; simpl; intros.
+destruct vals; inv H. auto.
+destruct a as [id ty]. destruct vals; try discriminate. auto.
+Qed. CloseFLemma.
+FLemma transl_vars_names:
+  forall ce vars tvars,
+  mmap (transl_var ce) vars = OK tvars ->
+  map fst tvars = S.var_names vars.
+FProofLemma.
+  intros. exploit mmap_inversion; eauto. generalize vars tvars. induction 1; simpl.
+- auto.
+- monadInv H0. simpl; congruence.
+Qed. CloseFLemma.
+
+FLemma function_ptr_translated
+  : forall prog tprog ge tge, match_prog prog tprog ->
+    ge = Genv.globalenv prog ->
+    tge = Genv.globalenv tprog ->
+    forall v f, 
+      Genv.find_funct_ptr ge v = Some f ->
+      exists cu tf, Genv.find_funct_ptr tge v = Some tf /\ match_fundef cu f tf /\ linkorder cu prog.
+FProofLemma.
+intros until tge. intros TRANSL A B.
+rewrite A. rewrite B.
+apply (Genv.find_funct_ptr_match TRANSL).
+Qed. CloseFLemma.
+
+FLemma symbols_preserved : 
+  forall prog tprog ge tge, match_prog prog tprog ->
+  ge = Genv.globalenv prog ->
+  tge = Genv.globalenv tprog ->
+  forall (s: ident), Genv.find_symbol tge s = Genv.find_symbol ge s.
+FProofLemma.
+intros until tge; intros TRANSL A B. rewrite A. rewrite B.
+apply (Genv.find_symbol_match TRANSL).
+Qed. CloseFLemma.
+
+(* ------------------------------------------------ *)
+(*               CORRECTNESS - EXPR                 *)
+(* ------------------------------------------------ *)
+FInduction transl_expr_correct about S.eval_expr 
+  motive (fun ge (e: S.env) le m a v (_ : S.eval_expr ge e le m a v) =>
+      forall prog tprog tge, match_prog prog tprog ->
+      S.globalenv prog = ge -> Genv.globalenv tprog = tge ->
+      forall (cunit: S.program) (L : linkorder cunit prog) te ta (MENV: match_env prog e te) lenv,
+      transl_expr a cunit.(prog_comp_env) = OK ta ->
+      T.eval_expr tge te le m lenv ta v).
+FProof.
+all: unfold transl_expr in *; unfold fst in *.
+(* const int *)
++ intros. fsimpl in H2. inv H2. apply make_intconst_correct.
+(* const float *)  
++ intros. fsimpl in H2. inv H2. apply make_floatconst_correct.
+(* const single *)  
++ intros. fsimpl in H2. inv H2. apply make_singleconst_correct.
+(* const long *)  
++ intros. fsimpl in H2. inv H2. apply make_longconst_correct.
+(* cast *)  
++ intros. fsimpl in H3. monadInv H3. eapply make_cast_correct; eauto.
+(* temp var *)  
++ intros. fsimpl in H2. monadInv H2. fconstructor.
+Qed. FEnd transl_expr_correct.
+(* ------------------------------------------------ *)
+(*              CORRECTNESS - OTHER1                *)
+(* ------------------------------------------------ *)
+FInductive match_transl
+  : self__Cshmgen.T.stmt -> self__Cshmgen.T.cont ->
+    self__Cshmgen.T.stmt -> self__Cshmgen.T.cont -> Prop :=
+| match_transl_0: forall ts tk,
+    match_transl ts tk ts tk.
+
+FInductive match_cont : composite_env -> type -> nat -> nat -> S.cont -> T.cont -> Prop :=
+| match_Kstop: forall ce tyret nbrk ncnt,
+    match_cont ce tyret nbrk ncnt S.Kstop T.Kstop      
+| match_Kseq: forall ce tyret nbrk ncnt s k ts tk,
+    transl_stmt s ce tyret nbrk ncnt = OK ts ->
+    match_cont ce tyret nbrk ncnt k tk ->
+    match_cont ce tyret nbrk ncnt (S.Kseq s k) (T.Kseq ts tk).
+               
+MetaData match_states.
+Inductive match_states (prog: S.program): S.state -> T.state -> Prop :=
+| match_state:
+    forall f nbrk ncnt s k e le m tf ts tk te ts' tk' (cu : S.program)
+        (LINK: linkorder cu prog)
+        (TRF: transl_function cu.(prog_comp_env) f = OK tf)
+        (TR: transl_stmt s cu.(prog_comp_env) (S.fn_return f) nbrk ncnt = OK ts)
+        (MTR: match_transl ts tk ts' tk')
+        (MENV: match_env prog e te)
+        (MK: match_cont cu.(prog_comp_env) (S.fn_return f) nbrk ncnt k tk),
+    match_states prog (S.State f s k e le m)
+      (T.State tf ts' tk' te le m)      
+| match_callstate:
+    forall fd args k m tfd tk targs tres cconv cu ce
+           (LINK: linkorder cu prog)
+        (TR: match_fundef cu fd tfd)
+        (MK: match_cont ce tres 0%nat 0%nat k tk)
+        (ISCC: S.is_call_cont k)
+        (TY: S.type_of_fundef fd = Tfunction targs tres cconv)
+        (CASTED: Val.has_argtype_list args (List.map argtype_of_type targs)),
+    match_states prog (S.Callstate fd args k m)
+      (T.Callstate tfd args tk m)      
+| match_returnstate:
+    forall res tres k m tk ce
+        (MK: match_cont ce tres 0%nat 0%nat k tk),
+        (* (WT: wt_val res tres),*) (* Need Ctyping.v? *)
+    match_states prog (S.Returnstate res k m)
+      (T.Returnstate res tk m).
+FEnd match_states.
+
+(* This should probably take tprog and match_prog as Hypothesis *)
+FLemma match_states_skip:
+  forall f e le te nbrk ncnt k tf tk m (cu: S.program) (prog: S.program),
+  linkorder cu prog ->
+  transl_function cu.(prog_comp_env) f = OK tf ->
+  match_env prog e te ->
+  match_cont cu.(prog_comp_env) (S.fn_return f) nbrk ncnt k tk ->
+  match_states prog (S.State f S.Sskip k e le m) (T.State tf T.Sskip tk te le m).
+FProofLemma.
+  intros. econstructor; eauto. fsimpl ; reflexivity. fconstructor.
+Qed. CloseFLemma.
+(* ------------------------------------------------ *)
+(*            CORRECTNESS - FIND_LABEL              *)
+(* ------------------------------------------------ *)
+(* ------------------------------------------------ *)
+(*              CORRECTNESS - OTHER2                *)
+(* ------------------------------------------------ *)
+FInduction match_cont_call_cont about match_cont 
+  motive (fun ce tyret nbrk ncnt k tk (_ : match_cont ce tyret nbrk ncnt k tk) =>
+  forall ce' nbrk' ncnt',
+  match_cont ce' tyret nbrk' ncnt' (S.call_cont k) (T.call_cont tk)).
+FProof.
++ intros. do 2 fsimpl. fconstructor.
++ intros until tk; intros A B H. do 2 fsimpl. apply H.
+Qed. FEnd match_cont_call_cont. 
+
+FInduction match_cont_is_call_cont about match_cont
+  motive (fun ce tyret nbrk ncnt k tk (_ : match_cont ce tyret nbrk ncnt k tk) =>
+  forall ce' nbrk' ncnt',
+  S.is_call_cont k ->
+  match_cont ce' tyret nbrk' ncnt' k tk /\ T.is_call_cont tk).
+FProof.
++ intros. fsimpl in *. fsimpl in H. split. fconstructor. auto.
++ intros. fsimpl in *. fsimpl in H0. contradiction.
+Qed. FEnd match_cont_is_call_cont.  
+
+(* use closing fact for inversion*)
+Closing Fact match_transl_0_inv :
+  forall ts tk ts' tk',
+    match_transl ts tk ts' tk' ->
+    ts' = ts /\ tk' = tk
+    by plain {intros until tmp; intros H; inv H; eauto}.
+
+Closing Fact match_Kseq_inv :
+  forall ce tyret nbrk ncnt s k the_tk,
+    match_cont ce tyret nbrk ncnt (S.Kseq s k) the_tk ->
+    exists ts tk,
+    the_tk = T.Kseq ts tk /\
+      transl_stmt s ce tyret nbrk ncnt = OK ts /\
+      match_cont ce tyret nbrk ncnt k tk
+    by plain {intros until the_tk; intros H; inv H; eauto}.
+
+Closing Fact match_Kstop_inv :
+  forall ce tyret nbrk ncnt tk,
+    match_cont ce tyret nbrk ncnt S.Kstop tk ->
+    tk = T.Kstop
+    by plain {intros until tmp; intros H; inv H; eauto}.
+
+FLemma transl_fundef_sig1:
+  forall ce f tf args res cc,
+  match_fundef ce f tf ->
+  Cop.classify_fun (S.type_of_fundef f) = fun_case_f args res cc ->
+  T.funsig tf = signature_of_type args res cc.
+FProofLemma.
+  intros. inv H.
+- monadInv H1. simpl. inversion H0. reflexivity.
+- simpl in H0. unfold T.funsig. congruence.
+Qed. CloseFLemma.
+
+FLemma transl_fundef_sig2:
+  forall ce f tf args res cc,
+  match_fundef ce f tf ->
+  S.type_of_fundef f = Tfunction args res cc ->
+  T.funsig tf = signature_of_type args res cc.
+FProofLemma.
+  intros. eapply transl_fundef_sig1; eauto.
+  rewrite H0; reflexivity.
+Qed. CloseFLemma.
+
+FInduction transl_find_label about S.stmt motive (fun (s : S.stmt) =>
+  forall ce lbl tyret nbrk ncnt k ts tk
+  (TR: transl_stmt s ce tyret nbrk ncnt = OK ts)
+  (MC: match_cont ce tyret nbrk ncnt k tk),
+  match S.find_label s lbl k with
+  | None => T.find_label ts lbl tk = None
+  | Some (s', k') =>
+      exists ts', exists tk', exists nbrk', exists ncnt',
+      T.find_label ts lbl tk = Some (ts', tk')
+      /\ transl_stmt s' ce tyret nbrk' ncnt' = OK ts'
+      /\ match_cont ce tyret nbrk' ncnt' k' tk'
+  end).
+FProof.
+all: intros; fsimpl in TR; try (monadInv TR); simpl; fsimpl.
+(* skip *)
++ fsimpl; reflexivity.
+(* assign *)  
++ fsimpl; reflexivity.
+(* seq *)  
++ exploit (H ce lbl tyret nbrk ncnt (S.Kseq __i k)); eauto. fconstructor.
+  destruct (S.find_label __i lbl (S.Kseq __i k)) as [[s' k'] | ].    
+  intros [ts' [tk' [nbrk' [ncnt' [A [B C]]]]]].
+  apply cheat.
+  apply cheat.
+  (*rewrite A. exists ts'; exists tk'; exists nbrk'; exists ncnt'; auto.
+  intro. rewrite H. eapply transl_find_label; eauto. *)
+(* ifthenelse *)  
++ exploit H; eauto. instantiate (1 := lbl).
+  destruct (S.find_label __i lbl k) as [[s' k'] | ].
+  intros [ts' [tk' [nbrk' [ncnt' [A [B C]]]]]].
+  (* rewrite A. exists ts'; exists tk'; exists nbrk'; exists ncnt'; auto.*)
+  apply cheat.
+  (* intro. rewrite H1. eapply transl_find_label; eauto.*)
+  (* where is x0 coming from? *)
+  apply cheat.
+(* return *)  
++ destruct o; monadInv TR; fsimpl; reflexivity.
+(* label *)  
++ destruct (ident_eq lbl l).
+  exists x; exists tk; exists nbrk; exists ncnt; auto. subst.
+  (* fsimpl. eapply H; eauto.*)
+  apply cheat.
+  eapply cheat.
+(* goto *)  
++ fsimpl; reflexivity.
+Qed. FEnd transl_find_label.
+
+FInduction transl_step about S.step
+  motive (fun ge S1 t S2 (_ : S.step ge S1 t S2) => 
+            forall prog tprog tge,
+            match_prog prog tprog ->
+           forall (A : S.globalenv prog = ge) (B : Genv.globalenv tprog = tge), 
+  forall T1, match_states prog S1 T1 -> 
+  exists T2, plus T.step tge T1 t T2 /\ match_states prog S2 T2).
+FProof.
+all: intros until tge; intros TRANSL A B; intros T1 MST; inv MST.
+(* skip seq *)
++ fsimpl in TR. monadInv TR. apply match_transl_0_inv in MTR; unpack MTR; subst.
+  apply match_Kseq_inv in MK; unpack MK. subst.  
+  econstructor; split.
+  apply plus_one. apply T.step_skip_seq.
+  econstructor; eauto. fconstructor.
+(* set *)  
++ fsimpl in TR.  monadInv TR. apply match_transl_0_inv in MTR; unpack MTR; subst. econstructor; split.
+  apply plus_one. fconstructor. eapply transl_expr_correct; eauto.
+  eapply match_states_skip; eauto.
+  (* letenv not used *)
+  Unshelve. apply nil.
+(* seq *)  
++ fsimpl in TR. monadInv TR. apply match_transl_0_inv in MTR; unpack MTR; subst.
+  econstructor; split.
+  apply plus_one. fconstructor.
+  econstructor; eauto. fconstructor.
+  fconstructor; eauto.
+(* ifthenelse *)  
++ fsimpl in TR. monadInv TR. apply match_transl_0_inv in MTR; unpack MTR; subst.
+  exploit make_boolean_correct; eauto.
+  exploit transl_expr_correct; eauto.
+  intros [v [A B]].
+  econstructor; split.
+  apply plus_one. apply T.step_ifthenelse with (v := v) (b := b) (lenv := nil); auto.
+  apply A. destruct b. econstructor; eauto. fconstructor. econstructor; eauto. fconstructor.
+(* return none *)  
++ fsimpl in TR. monadInv TR. apply match_transl_0_inv in MTR; unpack MTR; subst.
+  econstructor; split.
+  apply plus_one. fconstructor.
+  eapply match_env_free_blocks; eauto.
+  eapply match_returnstate with (ce := prog_comp_env cu); eauto.
+  eapply match_cont_call_cont. eauto.
+  (* constructor *)
+(* return some *)  
++ fsimpl in TR. monadInv TR. apply match_transl_0_inv in MTR; unpack MTR; subst.
+  econstructor; split.
+  apply plus_one. fconstructor.
+  eapply make_cast_correct; eauto. eapply transl_expr_correct; eauto.
+  eapply match_env_free_blocks; eauto.
+  eapply match_returnstate with (ce := prog_comp_env cu); eauto.
+  eapply match_cont_call_cont. eauto.
+  Unshelve. apply nil.
+  (* apply wt_val_casted. eapply cast_val_is_casted; eauto. *)
+(* skip call *)  
++ fsimpl in TR. monadInv TR. apply match_transl_0_inv in MTR; unpack MTR; subst.
+  exploit match_cont_is_call_cont; eauto. intros [A B].
+  econstructor; split.
+  apply plus_one. apply T.step_skip_call. auto.
+  eapply match_env_free_blocks; eauto.
+  eapply match_returnstate with (ce := prog_comp_env cu); eauto.
+  (* constructor.*)
+(* label *)  
++ fsimpl in TR. monadInv TR. apply match_transl_0_inv in MTR; unpack MTR; subst.
+  econstructor; split.
+  apply plus_one. fconstructor.
+  econstructor; eauto. fconstructor.
+  
+(* goto *)  
++ fsimpl in TR. monadInv TR. apply match_transl_0_inv in MTR; unpack MTR; subst.
+  generalize TRF. unfold transl_function. intro TRF'. monadInv TRF'.
+  exploit (transl_find_label (S.fn_body f) (prog_comp_env cu) lbl). eexact EQ. eapply match_cont_call_cont. eauto.
+  rewrite e0.
+  intros [ts' [tk'' [nbrk' [ncnt' [A [B C]]]]]].
+  econstructor; split.
+  apply plus_one. fconstructor. simpl. (* eexact A.*)
+  econstructor; eauto. fconstructor.
+  
+(* internal function *)  
++ inv f0. inv TR. monadInv H5. 
+  exploit match_cont_is_call_cont; eauto. intros [A B].
+  exploit match_env_alloc_variables; eauto.
+  apply match_env_empty.
+  intros [te1 [C D]].
+  simpl in TY. unfold S.type_of_function in TY.
+  econstructor; split.
+  apply plus_one. eapply T.step_internal_function.
+  simpl. replace (map snd (S.fn_params f)) with targs. exact CASTED.
+  unfold type_of_params in TY; congruence. 
+  simpl. erewrite transl_vars_names by eauto. assumption.
+  simpl. assumption.
+  simpl. assumption.
+  simpl; eauto.
+  simpl. rewrite create_undef_temps_match. eapply bind_parameter_temps_match; eauto.
+  simpl. econstructor; eauto.
+  unfold transl_function. rewrite EQ; simpl. rewrite EQ1; simpl. auto.
+  fconstructor.
+  replace (S.fn_return f) with tres. eassumption. congruence.
+Qed. FEnd transl_step.
+
+FLemma transl_initial_states:
+  forall S' ge tge prog tprog, match_prog prog tprog -> S.initial_state prog S' ->
+  ge = Genv.globalenv prog ->
+  tge = Genv.globalenv tprog ->                        
+  transl_program prog = OK tprog ->
+  exists R, T.initial_state tprog R /\ match_states prog S' R.
+FProofLemma.
+ intros. inv H0.
+ exploit function_ptr_translated; eauto. intros (cu & tf & A & B & C).
+ remember H as TRANSL.
+ assert (D: Genv.find_symbol (Genv.globalenv tprog) (AST.prog_main tprog) = Some b).
+ { destruct H as (P & Q & R). rewrite Q.
+   rewrite (symbols_preserved prog tprog (Genv.globalenv prog) (Genv.globalenv tprog) TRANSL eq_refl eq_refl). auto. }
+  assert (E: T.funsig tf = signature_of_type nil type_int32s cc_default).
+  { eapply transl_fundef_sig2; eauto. }
+  econstructor; split.
+  econstructor; eauto. apply (Genv.init_mem_match TRANSL). eauto.
+  econstructor; eauto. instantiate (1 := prog_comp_env cu). fconstructor; auto. fsimpl. exact I. constructor.
+Qed. CloseFLemma.          
+          
+FLemma transl_final_states:
+  forall S' R r prog,
+  match_states prog S' R -> S.final_state S' r -> T.final_state R r.
+FProofLemma.
+intros. inv H0. inv H. apply match_Kstop_inv in MK.
+subst. constructor.
+Qed. CloseFLemma.
 
 FEnd Cshmgen.
 
@@ -709,7 +2054,49 @@ Trait Clight_Sloop extends Clight.
 FInductive stmt : Type := 
   | Sloop: stmt -> stmt -> stmt (* infinite loop *)
   | Sbreak : stmt (* break statement *)
-  | Scontinue : stmt. (* continue statement *) 
+  | Scontinue : stmt. (* continue statement *)
+
+FInductive cont: Type :=
+| Kloop1: stmt -> stmt -> cont -> cont  (* Kloop1 s1 s2 k = after s1 in Sloop s1 s2 *)
+| Kloop2: stmt -> stmt -> cont -> cont. (* Kloop2 s1 s2 k = after s2 in Sloop s1 s2 *)
+
+FRecursion call_cont.
+Case Kloop1 s1 s2 k := (call_cont k).
+Case Kloop2 s1 s2 k := (call_cont k).
+FEnd call_cont.
+
+FRecursion is_call_cont.
+Case _ := False.
+FEnd is_call_cont.
+
+FRecursion find_label.
+Case Sloop s1 s2 :=
+  (fun lbl k =>
+     match find_label s1 lbl (Kloop1 s1 s2 k) with
+     | Some sk => Some sk
+     | None => find_label s2 lbl (Kloop2 s1 s2 k)
+     end).
+Case _ := (fun lbl k => None).
+FEnd find_label.
+
+FInductive step : genv -> state -> trace -> state -> Prop :=
+| step_loop: forall ge f s1 s2 k e le m,
+      step ge (State f (Sloop s1 s2) k e le m)
+        E0 (State f s1 (Kloop1 s1 s2 k) e le m)        
+| step_skip_or_continue_loop1: forall ge f s1 s2 k e le m x,
+      x = Sskip \/ x = Scontinue ->
+      step ge (State f x (Kloop1 s1 s2 k) e le m)
+        E0 (State f s2 (Kloop2 s1 s2 k) e le m)
+| step_break_loop1: forall ge f s1 s2 k e le m,
+      step ge (State f Sbreak (Kloop1 s1 s2 k) e le m)
+        E0 (State f Sskip k e le m)
+| step_skip_loop2: forall ge f s1 s2 k e le m,
+      step ge (State f Sskip (Kloop2 s1 s2 k) e le m)
+        E0 (State f (Sloop s1 s2) k e le m)
+| step_break_loop2: forall ge f s1 s2 k e le m,
+      step ge (State f Sbreak (Kloop2 s1 s2 k) e le m)
+        E0 (State f Sskip k e le m).
+  
 FEnd Clight_Sloop.
 
 Family Clight extends Clight_Sloop.
@@ -717,45 +2104,245 @@ FEnd Clight.
 
 Trait Csharpminor_Sblock extends Csharpminor.
 FInductive stmt : Type :=
-| Sblock: stmt -> stmt. 
+| Sblock: stmt -> stmt
+| Sexit: nat -> stmt.
+
+FInductive cont: Type :=
+| Kblock: cont -> cont.
+
+FRecursion call_cont.
+Case Kblock k := (call_cont k).
+FEnd call_cont.
+
+FRecursion is_call_cont.
+Case _ := False.
+FEnd is_call_cont.
+
+FRecursion find_label.
+Case Sblock s1 :=
+  (fun lbl k => find_label s1 lbl (Kblock k)).
+Case _ := (fun lbl k => None).
+FEnd find_label.
+
+FInductive step : genv -> state -> trace -> state -> Prop :=
+| step_block: forall ge f s k e le m,
+      step ge (State f (Sblock s) k e le m)
+        E0 (State f s (Kblock k) e le m)
+| step_skip_block: forall ge f k e le m,
+      step ge (State f Sskip (Kblock k) e le m)
+        E0 (State f Sskip k e le m)        
+| step_exit_seq: forall ge f n s k e le m,
+    step ge (State f (Sexit n) (Kseq s k) e le m)
+      E0 (State f (Sexit n) k e le m)
+| step_exit_block_0: forall ge f k e le m,
+    step ge (State f (Sexit O) (Kblock k) e le m)
+      E0 (State f Sskip k e le m)
+| step_exit_block_S: forall ge f n k e le m,
+    step ge (State f (Sexit (S n)) (Kblock k) e le m)
+      E0 (State f (Sexit n) k e le m).
+  
 FEnd Csharpminor_Sblock.
 
-Trait Csharpminor_Sexit extends Csharpminor.
+(*Trait Csharpminor_Sexit extends Csharpminor.
 FInductive stmt : Type :=
 | Sexit: nat -> stmt.
-FEnd Csharpminor_Sexit.
+FEnd Csharpminor_Sexit.*)
 
 Trait Csharpminor_Sloop extends Csharpminor.
 FInductive stmt : Type :=
 | Sloop: stmt -> stmt.
+
+FRecursion find_label.
+Case Sloop s1 :=
+  (fun lbl k => find_label s1 lbl (Kseq (Sloop s1) k)).
+FEnd find_label.
+
+FInductive step : genv -> state -> trace -> state -> Prop :=
+| step_loop: forall ge f s k e le m,
+      step ge (State f (Sloop s) k e le m)
+        E0 (State f s (Kseq (Sloop s) k) e le m).
+
 FEnd Csharpminor_Sloop.
 
 Family Csharpminor extends   
-  Csharpminor_Sexit, 
+  (* Csharpminor_Sexit, *)
   Csharpminor_Sloop,
   Csharpminor_Sblock.
 FEnd Csharpminor.
 
-From NFPOP Require Import Errors.
+From Rocqet Require Import Errors.
 Local Open Scope error_monad_scope.
 
-Trait Cshmgen_Sloop extends Cshmgen.
+Family Cshmgen.
 Family S extends Clight_Sloop. FEnd S.
+Family T extends Csharpminor. FEnd T.
 
-FRecursion transl_stmt with transl_lbl_stmt.
-
+FRecursion transl_stmt. (* with transl_lbl_stmt.*)
 Case Sloop s1 s2 :=
 (fun ce tyret nbrk ncnt =>
   do ts1 <- transl_stmt s1 ce tyret 1%nat 0%nat;
-  do ts2 <- transl_stmt s2 ce tyret 0%nat ((1 + ncnt)%nat);
+  do ts2 <- transl_stmt s2 ce tyret 0%nat (Datatypes.S ncnt);
   OK (T.Sblock (T.Sloop (T.Sseq (T.Sblock ts1) ts2)))).
 Case Sbreak := (fun ce tyret nbrk ncnt => OK (T.Sexit nbrk)).
 Case Scontinue := (fun ce tyret nbrk ncnt => OK (T.Sexit ncnt)).
-FEnd transl_stmt with transl_lbl_stmt.
+FEnd transl_stmt. (* with transl_lbl_stmt.*)
 
-FEnd Cshmgen_Sloop.
+FInductive match_transl
+  : T.stmt -> T.cont ->
+    T.stmt -> T.cont -> Prop :=
+| match_transl_1: forall ts tk,
+    match_transl (T.Sblock ts) tk ts (T.Kblock tk).
 
-Family Cshmgen extends Cshmgen_Sloop.
+FDefinition Succ := Datatypes.S.
+
+FInductive match_cont : composite_env -> type -> nat -> nat -> S.cont -> T.cont -> Prop :=               
+| match_Kloop1: forall ce tyret s1 s2 k ts1 ts2 nbrk ncnt tk,
+    transl_stmt s1 ce tyret 1%nat 0%nat = OK ts1 ->
+    transl_stmt s2 ce tyret 0%nat (Succ ncnt) = OK ts2 ->
+    match_cont ce tyret nbrk ncnt k tk ->
+    match_cont ce tyret 1%nat 0%nat
+               (S.Kloop1 s1 s2 k)
+               (T.Kblock
+                  (T.Kseq ts2
+                     (T.Kseq
+                        (T.Sloop
+                           (T.Sseq
+                              (T.Sblock ts1) ts2))
+                        (T.Kblock tk))))
+| match_Kloop2: forall ce tyret s1 s2 k ts1 ts2 nbrk ncnt tk,
+    transl_stmt s1 ce tyret 1%nat 0%nat = OK ts1 ->
+    transl_stmt s2 ce tyret 0%nat (Succ ncnt) = OK ts2 ->
+    match_cont ce tyret nbrk ncnt k tk ->
+    match_cont ce tyret 0%nat (Succ ncnt)
+               (S.Kloop2 s1 s2 k)
+               (T.Kseq
+                  (T.Sloop
+                     (T.Sseq
+                        (T.Sblock ts1) ts2))
+                  (T.Kblock tk)).
+
+Closing Fact match_Kloop1_inv : forall ce tyret nbrk ncnt s1 s2 k tk,
+    match_cont ce tyret nbrk ncnt (S.Kloop1 s1 s2 k) tk ->
+    exists nbrk' ncnt' ts1 ts2 tk',
+       nbrk = 1%nat /\ ncnt = 0%nat /\
+       tk =  (T.Kblock (T.Kseq ts2 (T.Kseq (T.Sloop (T.Sseq (T.Sblock ts1) ts2)) (T.Kblock tk')))) /\
+       transl_stmt s1 ce tyret 1%nat 0%nat = OK ts1 /\
+       transl_stmt s2 ce tyret 0%nat (Succ ncnt') = OK ts2 /\
+       match_cont ce tyret nbrk' ncnt' k tk'
+by plain { apply cheat }.
+
+Closing Fact match_Kloop2_inv : forall ce tyret nbrk ncnt s1 s2 k tk,
+  match_cont ce tyret nbrk ncnt (S.Kloop2 s1 s2 k) tk ->
+  exists ncnt' nbrk' tk' ts1 ts2,
+    nbrk = 0%nat /\ ncnt = (Succ ncnt') /\
+    tk = (T.Kseq (T.Sloop (T.Sseq (T.Sblock ts1) ts2)) (T.Kblock tk')) /\
+    transl_stmt s1 ce tyret 1%nat 0%nat = OK ts1 /\
+    transl_stmt s2 ce tyret 0%nat (Succ ncnt') = OK ts2 /\
+    match_cont ce tyret nbrk' ncnt' k tk'
+by plain { apply cheat }.
+               
+FInduction match_cont_call_cont.
+FProof.
+all: intros; do 5 fsimpl; auto.
+Qed. FEnd match_cont_call_cont.
+
+FInduction match_cont_is_call_cont.
+FProof.
+all: intros; fsimpl in H0; contradiction. 
+Qed. FEnd match_cont_is_call_cont.
+
+FInduction transl_find_label.
+FProof.
+all: intros; fsimpl in TR; try (monadInv TR); simpl; fsimpl.
+(* loop *)
++ exploit (H ce lbl tyret 1%nat 0%nat (S.Kloop1 __i __i0 k)); eauto. fconstructor; eauto.
+  destruct (S.find_label __i lbl (S.Kloop1 __i __i0 k)) as [[s' k'] | ].
+  intros [ts' [tk' [nbrk' [ncnt' [A [B C]]]]]].  
+  (*rewrite A. exists ts'; exists tk'; exists nbrk'; exists ncnt'; auto.
+  intro. rewrite H.
+  eapply transl_find_label; eauto. econstructor; eauto.*)
+  apply cheat.
+  apply cheat.
+(* break *)  
++ fsimpl; reflexivity.
+(* continue *)
++ fsimpl; reflexivity.
+Qed. FEnd transl_find_label.
+
+Closing Fact match_transl_1_inv :
+  forall ts ts' tk tk', 
+    match_transl (T.Sblock ts) tk ts' tk' ->
+    ts' = ts /\
+    tk' = (T.Kblock tk)
+by plain { apply cheat }.                
+
+Closing Fact match_transl_step:
+  forall ts tk ts' tk' f te le m tge,
+  match_transl (T.Sblock ts) tk ts' tk' ->
+  star T.step tge (T.State f ts' tk' te le m) E0 (T.State f ts (T.Kblock tk) te le m)
+by plain { apply cheat }.       
+
+(*FLemma match_transl_step:
+  forall ts tk ts' tk' f te le m tge,
+  match_transl (T.Sblock ts) tk ts' tk' ->
+  star T.step tge (T.State f ts' tk' te le m) E0 (T.State f ts (T.Kblock tk) te le m).
+FProofLemma.
+  intros. apply match_transl_0_inv in H; unpack H. 
+  apply star_one. constructor.
+  apply star_refl.
+Qed.*)
+
+
+FInduction transl_step.
+FProof.
+all: intros until tge; intros TRANSL A B; intros T1 MST; inv MST.
+(* loop *)
++ fsimpl in TR. monadInv TR.
+  econstructor; split.
+  eapply star_plus_trans. eapply match_transl_step; eauto.
+  eapply plus_left. fconstructor.
+  eapply star_left. fconstructor.
+  apply star_one. fconstructor.
+  reflexivity. reflexivity. traceEq.
+  econstructor; eauto. fconstructor. fconstructor; eauto.
+  
+(* skip-or-continue loop *)  
++  assert ((ts' = T.Sskip \/ ts' = T.Sexit ncnt) /\ tk' = tk).
+   { destruct o; subst x; fsimpl in TR; monadInv TR; apply match_transl_0_inv in MTR; unpack MTR; subst; auto. }
+  destruct H. apply match_Kloop1_inv in MK; unpack MK; subst.
+  econstructor; split.
+  eapply plus_left.
+  destruct H; subst ts'. 2:fconstructor. fconstructor.
+  apply star_one. fconstructor. traceEq.
+  econstructor; eauto. fconstructor. fconstructor; eauto.
+  
+(* break loop1*)  
++  fsimpl in TR. monadInv TR. apply match_transl_0_inv in MTR; unpack MTR; subst. apply match_Kloop1_inv in MK; unpack MK; subst.
+  econstructor; split.
+  eapply plus_left. fconstructor.
+  eapply star_left. fconstructor.
+  eapply star_left. fconstructor.
+  apply star_one. fconstructor.
+  reflexivity. reflexivity. traceEq.
+  eapply match_states_skip; eauto.
+
+(* skip loop2 *)  
++ fsimpl in TR. monadInv TR. apply match_transl_0_inv in MTR; unpack MTR; subst. apply match_Kloop2_inv in MK; unpack MK; subst.
+  econstructor; split.
+  apply plus_one. fconstructor.
+  econstructor; eauto.
+  fsimpl. rewrite TEMP2; simpl. unfold Succ in TEMP3. rewrite TEMP3; simpl. eauto.
+  fconstructor.
+
+(* break loop2 *)    
++ fsimpl in TR. monadInv TR. apply match_transl_0_inv in MTR; unpack MTR; subst. apply match_Kloop2_inv in MK; unpack MK; subst. 
+  econstructor; split.
+  eapply plus_left. fconstructor.
+  apply star_one. fconstructor.
+  traceEq.
+  eapply match_states_skip; eauto.
+Qed. FEnd transl_step.
+
 FEnd Cshmgen.
 
 FEnd Comp_Loops.
@@ -765,14 +2352,80 @@ Trait Comp_Builtin extends Base.
 Family Clight.
 FInductive stmt : Type :=
 | Sbuiltin: option ident -> external_function -> list type -> list expr -> stmt. (* builtin invocation *)
+
+FRecursion find_label.
+Case _ := (fun lbl k => None).
+FEnd find_label.
+
+Inherit eval_expr.
+
+MetaData eval_exprlist binds eval_Enil, eval_Econs.
+Inductive eval_exprlist: genv -> env -> temp_env -> mem -> list expr -> list type -> list val -> Prop :=
+| eval_Enil: forall ge e le m,
+    eval_exprlist ge e le m nil nil nil
+| eval_Econs: forall ge e le m a bl ty tyl v1 v2 vl,
+    eval_expr ge e le m a v1 ->
+    Cop.sem_cast v1 (typeof a) ty m = Some v2 ->
+    eval_exprlist ge e le m bl tyl vl ->
+    eval_exprlist ge e le m (a :: bl) (ty :: tyl) (v2 :: vl).
+FEnd eval_exprlist.
+
+FDefinition set_opttemp := fun (optid: option ident) (v: val) (le: temp_env) =>
+  match optid with
+  | None => le
+  | Some id => PTree.set id v le
+  end.
+
+FInductive step : genv -> state -> trace -> state -> Prop :=
+| step_builtin: forall ge f optid ef tyargs al k e le m vargs t vres m',
+      eval_exprlist ge e le m al tyargs vargs ->
+      external_call ef (Genv.to_senv (self__Clight.genv_genv ge)) vargs m t vres m' ->
+      step ge (State f (Sbuiltin optid ef tyargs al) k e le m)
+         t (State f Sskip k e (set_opttemp optid vres le) m').
+  
 FEnd Clight.
 
-Family Csharpminor.
+Family Cfam.
+
+Inherit env.
+
+FDefinition set_optvar := fun (optid: option ident) (v: val) (e: env) =>
+  match optid with
+  | None => e
+  | Some id => PTree.set id v e
+  end.
+
+FEnd Cfam.
+
+Family Csharpminor extends Cfam.
 FInductive stmt : Type :=
-| Sbuiltin : option ident -> external_function -> list expr -> stmt.
+  | Sbuiltin : option ident -> external_function -> list expr -> stmt.
+
+Inherit eval_expr.
+
+MetaData eval_exprlist binds eval_Enil, eval_Econs.
+Inductive eval_exprlist: genv -> fenv -> env -> mem -> letenv -> list expr -> list val -> Prop :=
+  | eval_Enil: forall ge lenv e le m,
+      eval_exprlist ge le e m lenv nil nil
+  | eval_Econs: forall ge le e m lenv a1 al v1 vl,
+      eval_expr ge le e m lenv a1 v1 -> eval_exprlist ge le e m lenv al vl ->
+      eval_exprlist ge le e m lenv (a1 :: al) (v1 :: vl).
+FEnd eval_exprlist.
+
+FRecursion find_label.
+Case _ := (fun lbl k => None).
+FEnd find_label.
+
+FInductive step : genv -> state -> trace -> state -> Prop :=
+| step_builtin: forall ge f lenv optid ef bl k e le m vargs t vres m',
+      eval_exprlist ge e le m lenv bl vargs ->
+      external_call ef ge vargs m t vres m' ->
+      step ge (State f (Sbuiltin optid ef bl) k e le m)
+        t (State f Sskip k e (set_optvar optid vres le) m').
+        
 FEnd Csharpminor.
 
-From NFPOP Require Import Errors.
+From Rocqet Require Import Errors.
 Local Open Scope error_monad_scope.
 
 Family Cshmgen.
@@ -785,7 +2438,7 @@ Fixpoint transl_arglist (ce: composite_env) (al: list self__Cshmgen.S.expr) (tyl
   match al, tyl with
   | nil, nil => OK nil
   | a1 :: a2, ty1 :: ty2 =>
-      do ta1 <- self__Cshmgen.transl_expr a1 ce;
+      do ta1 <- transl_expr a1 ce;
       do ta1' <- self__Cshmgen.make_cast (self__Cshmgen.S.typeof a1) ty1 ta1;
       do ta2 <- transl_arglist ce a2 ty2;
       OK (ta1' :: ta2)
@@ -799,70 +2452,214 @@ Fixpoint transl_arglist (ce: composite_env) (al: list self__Cshmgen.S.expr) (tyl
   end.
 FEnd transl_arglist.
 
-FRecursion transl_stmt with transl_lbl_stmt.
+FRecursion transl_stmt.
 Case Sbuiltin x ef tyargs bl :=
 (fun ce tyret nbrk ncnt =>
   do tbl <- transl_arglist ce bl tyargs;
   OK(T.Sbuiltin x ef tbl)).
-FEnd transl_stmt with transl_lbl_stmt.
+FEnd transl_stmt.
+
+FInduction transl_find_label.
+FProof.
+all: intros; fsimpl in TR; try (monadInv TR); simpl; fsimpl.
++ fsimpl; reflexivity.
+Qed. FEnd transl_find_label.
+
+FLemma transl_arglist_correct:
+  forall (cunit: S.program) prog tprog (LINK : linkorder cunit prog) al tyl vl ge tge e te le m lenv
+         (MENV: match_env prog e te),
+  match_prog prog tprog ->    
+  S.globalenv prog = ge -> Genv.globalenv tprog = tge ->  
+  S.eval_exprlist ge e le m al tyl vl ->
+  forall tal, transl_arglist cunit.(prog_comp_env) al tyl = OK tal ->
+  T.eval_exprlist tge te le m lenv tal vl.
+FProofLemma.
+  induction 6; intros.
+  monadInv H2. constructor.
+  monadInv H5. constructor.
+  eapply make_cast_correct; eauto. eapply transl_expr_correct; eauto. auto.
+Qed. CloseFLemma.
+
+FLemma senv_preserved: forall prog tprog ge tge, match_prog prog tprog ->
+  ge = Genv.globalenv prog ->
+  tge = Genv.globalenv tprog ->
+  Senv.equiv (Genv.to_senv ge) (Genv.to_senv tge).
+FProofLemma.
+intros until tge; intros TRANSL A B. rewrite A. rewrite B.
+apply (Genv.senv_match TRANSL).
+Qed. CloseFLemma.
+
+FInduction transl_step.
+FProof.
+all: intros until tge; intros TRANSL A B; intros T1 MST; inv MST.
++ fsimpl in TR. monadInv TR. apply match_transl_0_inv in MTR; unpack MTR; subst.
+  econstructor; split.
+  apply plus_one. fconstructor.
+  eapply transl_arglist_correct; eauto.
+  eapply external_call_symbols_preserved with (ge1 := (Genv.to_senv (S.genv_genv (S.globalenv prog)))).
+  apply (senv_preserved prog tprog (Genv.globalenv prog) (Genv.globalenv tprog) TRANSL eq_refl eq_refl).  eauto.
+  eapply match_states_skip; eauto.
+  Unshelve. apply nil.  
+Qed. FEnd transl_step.
+
 FEnd Cshmgen.
 
 FEnd Comp_Builtin.
 
 Trait Comp_Heap extends Base, Comp_Builtin.
 
-Trait Clight_Evar extends Clight.
+Trait Clight_Lvalues extends Clight.
 FInductive expr : Type :=
-| Evar: ident -> type -> expr. (* variable *)
-
-FRecursion typeof.
-Case Evar i t := t.
-FEnd typeof.
-FEnd Clight_Evar.
-
-Trait Clight_Ederef extends Clight.
-FInductive expr : Type :=
-| Ederef: expr -> type -> expr. (* pointer dereference (unary *)
-
-FRecursion typeof.
-Case Ederef i t := t.
-FEnd typeof.
-FEnd Clight_Ederef.
-
-Trait Clight_Eaddrof extends Clight.
-FInductive expr : Type :=
+| Evar: ident -> type -> expr (* variable *)
+| Ederef: expr -> type -> expr (* pointer dereference (unary *)                             
 | Eaddrof: expr -> type -> expr. (* address-of operator (&) *)
 
 FRecursion typeof.
+Case Evar i t := t.
 Case Eaddrof e t := t.
+Case Ederef i t := t.
 FEnd typeof.
-FEnd Clight_Eaddrof.
 
-Trait Clight_Sassign extends Clight.
+MetaData deref_loc.
+Inductive deref_loc (ty: type) (m: mem) (b: block) (ofs: ptrofs) :
+                                             bitfield -> val -> Prop :=
+  | deref_loc_value: forall chunk v,
+      access_mode ty = By_value chunk ->
+      Mem.loadv chunk m (Vptr b ofs) = Some v ->
+      deref_loc ty m b ofs Full v
+  | deref_loc_reference:
+      access_mode ty = By_reference ->
+      deref_loc ty m b ofs Full (Vptr b ofs)
+  | deref_loc_copy:
+      access_mode ty = By_copy ->
+      deref_loc ty m b ofs Full (Vptr b ofs)
+  | deref_loc_bitfield: forall sz sg pos width v,
+      load_bitfield ty sz sg pos width m (Vptr b ofs) v ->
+      deref_loc ty m b ofs (Bits sz sg pos width) v.
+FEnd deref_loc.
+
+FInductive eval_expr : genv -> env -> temp_env -> mem -> expr -> val -> Prop :=
+| eval_Eaddrof: forall ge e le m a ty loc ofs,
+   eval_lvalue ge e le m a loc ofs Ctypes.Full ->
+   eval_expr ge e le m (Eaddrof a ty) (Vptr loc ofs)
+| eval_Elvalue: forall ge e le m a loc ofs bf v,
+      eval_lvalue ge e le m a loc ofs bf ->
+      deref_loc (typeof a) m loc ofs bf v ->
+      eval_expr ge e le m a v             
+with eval_lvalue: genv -> env -> temp_env -> mem -> expr -> block -> ptrofs -> bitfield -> Prop :=
+  | eval_Evar_local: forall ge e le m id l ty,
+      e!id = Some(l, ty) ->
+      eval_lvalue ge e le m (Evar id ty) l Ptrofs.zero Ctypes.Full                  
+  | eval_Evar_global: forall ge e le m id l ty,
+      e!id = None ->
+      Genv.find_symbol (self__Clight_Lvalues.genv_genv ge) id = Some l ->
+      eval_lvalue ge e le m (Evar id ty) l Ptrofs.zero Ctypes.Full
+  | eval_Ederef: forall ge e le m a ty l ofs,
+      eval_expr ge e le m a (Vptr l ofs) ->
+      eval_lvalue ge e le m (Ederef a ty) l ofs Ctypes.Full.
+             
+FEnd Clight_Lvalues.
+
+Trait Clight_Sassign extends Clight, Clight_Lvalues.
 FInductive stmt : Type :=
 | Sassign : expr -> expr -> stmt. (* assignment lvalue = rvalue *)
+
+FRecursion find_label.
+Case _ := (fun lbl k => None).
+FEnd find_label.
+
+MetaData assign_loc.
+Inductive assign_loc (ce: composite_env) (ty: type) (m: mem) (b: block) (ofs: ptrofs):
+                                            bitfield -> val -> mem -> Prop :=
+  | assign_loc_value: forall v chunk m',
+      access_mode ty = By_value chunk ->
+      Mem.storev chunk m (Vptr b ofs) v = Some m' ->
+      assign_loc ce ty m b ofs Full v m'
+  | assign_loc_copy: forall b' ofs' bytes m',
+      access_mode ty = By_copy ->
+      (sizeof ce ty > 0 -> (alignof_blockcopy ce ty | Ptrofs.unsigned ofs')) ->
+      (sizeof ce ty > 0 -> (alignof_blockcopy ce ty | Ptrofs.unsigned ofs)) ->
+      b' <> b \/ Ptrofs.unsigned ofs' = Ptrofs.unsigned ofs
+              \/ Ptrofs.unsigned ofs' + sizeof ce ty <= Ptrofs.unsigned ofs
+              \/ Ptrofs.unsigned ofs + sizeof ce ty <= Ptrofs.unsigned ofs' ->
+      Mem.loadbytes m b' (Ptrofs.unsigned ofs') (sizeof ce ty) = Some bytes ->
+      Mem.storebytes m b (Ptrofs.unsigned ofs) bytes = Some m' ->
+      assign_loc ce ty m b ofs Full (Vptr b' ofs') m'
+  | assign_loc_bitfield: forall sz sg pos width v m' v',
+      store_bitfield ty sz sg pos width m (Vptr b ofs) v m' v' ->
+      assign_loc ce ty m b ofs (Bits sz sg pos width) v m'.
+FEnd assign_loc.
+
+FInductive step : genv -> state -> trace -> state -> Prop :=  
+| step_assign: forall ge f a1 a2 k e le m loc ofs bf v2 v m',
+      eval_lvalue ge e le m a1 loc ofs bf ->
+      eval_expr ge e le m a2 v2 ->
+      Cop.sem_cast v2 (typeof a2) (typeof a1) m = Some v ->
+      assign_loc (self__Clight_Sassign.genv_cenv ge) (typeof a1) m loc ofs bf v m' ->
+      step ge (State f (Sassign a1 a2) k e le m)
+        E0 (State f Sskip k e le m').
+
 FEnd Clight_Sassign.
 
 Family Clight extends 
-  Clight_Sassign, 
-  Clight_Eaddrof,
-  Clight_Ederef,
-  Clight_Evar.
+  Clight_Sassign,   
+  Clight_Lvalues.
 FEnd Clight.
 
 Trait Csharpminor_Eaddrof extends Csharpminor.
 FInductive expr : Type :=
 | Eaddrof : ident -> expr. (* taking the address of a variable *)
+
+Inherit letenv.
+
+MetaData eval_var_addr.
+Inductive eval_var_addr: genv -> fenv -> ident -> block -> Prop :=
+  | eval_var_addr_local:
+      forall ge e id b sz,
+      PTree.get id e = Some (b, sz) ->
+      eval_var_addr ge e id b
+  | eval_var_addr_global:
+      forall ge e id b,
+      PTree.get id e = None ->
+      Genv.find_symbol ge id = Some b ->
+      eval_var_addr ge e id b.
+FEnd eval_var_addr.
+
+FInductive eval_expr :  genv -> fenv -> env -> mem -> letenv -> expr -> val -> Prop :=
+| eval_Eaddrof: forall ge le e lenv m id b,
+      eval_var_addr ge le id b ->
+      eval_expr ge le e m lenv (Eaddrof id) (Vptr b Ptrofs.zero).
+                
 FEnd Csharpminor_Eaddrof.
 
 Trait Csharpminor_Eload extends Csharpminor.
 FInductive expr : Type :=
 | Eload : memory_chunk -> expr -> expr. (* memory read *)
+
+FInductive eval_expr :  genv -> fenv -> env -> mem -> letenv -> expr -> val -> Prop :=
+| eval_Eload: forall ge le e lenv m chunk a v1 v,
+      eval_expr ge le e m lenv a v1 ->
+      Mem.loadv chunk m v1 = Some v ->
+      eval_expr ge le e m lenv (Eload chunk a) v.
+  
 FEnd Csharpminor_Eload.
 
-Trait Csharpminor_Sstore extends Csharpminor.                                
+Trait Csharpminor_Sstore extends Csharpminor.
 FInductive stmt : Type :=
 | Sstore : memory_chunk -> expr -> expr -> stmt.
+
+FRecursion find_label.
+Case _ := (fun lbl k => None).
+FEnd find_label.
+
+FInductive step : genv -> state -> trace -> state -> Prop :=
+| step_store: forall ge f chunk addr a k e le m vaddr v m' lenv,
+      eval_expr ge e le m lenv addr vaddr ->
+      eval_expr ge e le m lenv a v ->
+      Mem.storev chunk m vaddr v = Some m' ->
+      step ge (State f (Sstore chunk addr a) k e le m)
+        E0 (State f Sskip k e le m').
+  
 FEnd Csharpminor_Sstore.
 
 Family Csharpminor extends 
@@ -871,11 +2668,12 @@ Family Csharpminor extends
   Csharpminor_Eaddrof.
 FEnd Csharpminor.
 
-Trait Cshmgen_Sassign extends Cshmgen.
-Family S extends Clight_Sassign. FEnd S.
+Family Cshmgen.
+Family S extends Clight. FEnd S.
+Family T extends Csharpminor. FEnd T.
 
 Inherit alignof.
-From NFPOP Require Import Errors.
+From Rocqet Require Import Errors.
 Local Open Scope error_monad_scope.
 
 FDefinition make_store_bitfield : intsize -> signedness -> Z -> Z -> T.expr -> T.expr -> res T.stmt := 
@@ -908,53 +2706,6 @@ FDefinition make_store := fun (ce: composite_env) (addr: T.expr) (ty: type) (bf:
   | Bits sz sg pos width =>
       make_store_bitfield sz sg pos width addr rhs
   end.
-
-FRecursion make_cmpu_ne_zero.
-Case Eaddrof v := (T.Ebinop (Ocmpu Cne) (T.Eaddrof v) (make_intconst Int.zero)).
-Case Eload ck e := (T.Ebinop (Ocmpu Cne) (T.Eload ck e) (make_intconst Int.zero)).
-FEnd make_cmpu_ne_zero.
-
-FOpaque Definition transl_lvalue :
-  composite_env -> S.expr -> res (T.expr * bitfield) := cheat.
-
-FRecursion transl_stmt with transl_lbl_stmt.
-Case Sassign b c :=
-(fun ce tyret nbrk ncnt => 
-   do (tb, bf) <- transl_lvalue ce b;
-   do tc <- transl_expr c ce;
-   do tc' <- make_cast (S.typeof c) (S.typeof b) tc;
-   make_store ce tb (S.typeof b) bf tc').
-FEnd transl_stmt with transl_lbl_stmt.
-
-FEnd Cshmgen_Sassign.
-
-Trait Cshmgen_Eaddrof extends Cshmgen.
-Family S extends Clight_Eaddrof. FEnd S.
-
-FRecursion make_cmpu_ne_zero.
-Case Eaddrof v := (T.Ebinop (Ocmpu Cne) (T.Eaddrof v) (make_intconst Int.zero)).
-Case Eload ck e := (T.Ebinop (Ocmpu Cne) (T.Eload ck e) (make_intconst Int.zero)).
-FEnd make_cmpu_ne_zero.
-
-FOpaque Definition transl_lvalue :
-  composite_env -> S.expr -> res (T.expr * bitfield) := cheat.
-
-FRecursion transl_expr.
-Case Eaddrof b c :=
-(fun ce => 
-   do (tb, bf) <- transl_lvalue ce b;
-   match bf with
-   | Full => OK tb
-   | Bits _ _ _ _ => Error (msg "Cshmgen.transl_expr: addrof bitfield")
-   end).
-FEnd transl_expr.
-
-FEnd Cshmgen_Eaddrof.
-
-Trait Cshmgen_Ederef_Evar extends Cshmgen.
-Family S extends Clight_Ederef, Clight_Evar. FEnd S.
-
-Inherit alignof.
 
 FDefinition make_extract_bitfield 
  : intsize -> signedness -> Z -> Z -> T.expr -> res T.expr := 
@@ -989,21 +2740,279 @@ Case Eaddrof v := (T.Ebinop (Ocmpu Cne) (T.Eaddrof v) (make_intconst Int.zero)).
 Case Eload ck e := (T.Ebinop (Ocmpu Cne) (T.Eload ck e) (make_intconst Int.zero)).
 FEnd make_cmpu_ne_zero.
 
-FRecursion transl_expr.
+FRecursion translate_expression.
+Case Eaddrof b c :=
+(fun ce => 
+   (do (tb, bf) <- snd (translate_expression b ce); (* transl_lvalue *)
+   match bf with
+   | Full => OK tb
+   | Bits _ _ _ _ => Error (msg "Cshmgen.transl_expr: addrof bitfield")
+   end,
+   Error(msg "Cshmgen.transl_lvalue"))).
 Case Ederef b ty :=
 (fun ce => 
-  do tb <- transl_expr b ce;
-      make_load tb ty Full).
+  (do tb <- fst (translate_expression b ce);
+   make_load tb ty Full,
+   do tb <- fst (translate_expression b ce);
+   OK (tb, Full))).
 Case Evar id ty :=
-   (fun ce => make_load (T.Eaddrof id) ty Full).
-FEnd transl_expr.
+   (fun ce => (make_load (T.Eaddrof id) ty Full, OK (T.Eaddrof id, Full))).
+FEnd translate_expression.
 
-FEnd Cshmgen_Ederef_Evar.
+FDefinition transl_lvalue := fun e ce => snd (translate_expression e ce).
 
-Family Cshmgen extends 
-  Cshmgen_Ederef_Evar, 
-  Cshmgen_Eaddrof, 
-  Cshmgen_Sassign.
+FRecursion transl_stmt.
+Case Sassign b c :=
+(fun ce tyret nbrk ncnt => 
+   do (tb, bf) <- transl_lvalue b ce;
+   do tc <- transl_expr c ce;
+   do tc' <- make_cast (S.typeof c) (S.typeof b) tc;
+   make_store ce tb (S.typeof b) bf tc').
+FEnd transl_stmt.
+
+FInduction make_cmpu_ne_zero_correct.
+FProof.
++ apply cheat.
++ apply cheat.  
+Qed. FEnd make_cmpu_ne_zero_correct.
+
+FInduction make_cmpu_ne_zero_correct_ptr.
+FProof.
++ apply cheat.
++ apply cheat.
+Qed. FEnd make_cmpu_ne_zero_correct_ptr.
+
+Inherit match_env.
+
+FLemma match_env_globals:
+  forall prog e te id,
+  match_env prog e te ->
+  e!id = None ->
+  te!id = None.
+FProofLemma.
+  intros. destruct (te!id) as [[b sz] | ] eqn:?; auto.
+  exploit me_local_inv; eauto. intros [ty EQ]. congruence.
+Qed. CloseFLemma.
+
+FInduction transl_expr_lvalue about S.eval_lvalue
+  motive (fun ge (e: S.env) le m a b ofs bf (_ : S.eval_lvalue ge e le m a b ofs bf) =>
+    forall prog tprog tge, match_prog prog tprog ->
+    S.globalenv prog = ge -> Genv.globalenv tprog = tge ->
+    forall (cunit: S.program) (L : linkorder cunit prog) te ta (MENV: match_env prog e te),
+    transl_expr a cunit.(prog_comp_env) = OK ta ->
+    exists tb, transl_lvalue a cunit.(prog_comp_env) = OK (tb, bf)
+               /\ make_load tb (S.typeof a) bf = OK ta).
+FProof.
+all: unfold transl_expr in *; unfold transl_lvalue in *; unfold snd in *; unfold fst in *.
+(* var local *)
++ intros. fsimpl in H2. exists (T.Eaddrof id); auto. do 2 fsimpl. auto.
+(* var global *)  
++ intros. fsimpl in H2. exists (T.Eaddrof id); auto. do 2 fsimpl. auto.
+(* deref *)  
++ intros. fsimpl in H2. monadInv H2. unfold fst in *. do 2 fsimpl. unfold fst. rewrite EQ. exists x; auto. 
+Qed. FEnd transl_expr_lvalue.  
+
+FLemma first_bit_range: forall sz pos width,
+  0 <= pos -> 0 < width -> pos + width <= bitsize_carrier sz ->
+     0 <= first_bit sz pos width < Int.zwordsize
+  /\ 0 <= Int.zwordsize - first_bit sz pos width - width < Int.zwordsize.
+FProofLemma.
+  intros.
+  assert (bitsize_carrier sz <= Int.zwordsize) by (destruct sz; compute; congruence).
+  unfold first_bit; destruct Archi.big_endian; lia.
+Qed. CloseFLemma.
+
+FLemma int_ltu_true:
+  forall x, 0 <= x < Int.zwordsize -> Int.ltu (Int.repr x) Int.iwordsize = true.
+FProofLemma.
+  intros. unfold Int.ltu. rewrite Int.unsigned_repr_wordsize, Int.unsigned_repr, zlt_true by (generalize Int.wordsize_max_unsigned; lia).
+  auto.
+Qed. CloseFLemma.
+
+FLemma make_load_correct:
+  forall ge addr ty bf code b ofs v e le m lenv,
+  make_load addr ty bf = OK code ->
+  T.eval_expr ge e le m lenv addr (Vptr b ofs) ->
+  S.deref_loc ty m b ofs bf v ->
+  T.eval_expr ge e le m lenv code v.
+FProofLemma.
+  unfold make_load; intros until lenv; intros MKLOAD EVEXP DEREF.
+  inv DEREF.
+- (* scalar *)
+  rewrite H in MKLOAD. inv MKLOAD. apply T.eval_Eload with (Vptr b ofs); auto.
+- (* by reference *)
+  rewrite H in MKLOAD. inv MKLOAD. auto.
+- (* by copy *)
+  rewrite H in MKLOAD. inv MKLOAD. auto.
+- (* by bitfield *)
+  inv H.
+  unfold make_extract_bitfield in MKLOAD. unfold bitfield_extract.
+  exploit (first_bit_range sz pos width); eauto. lia. intros [A1 A2].
+  set (amount1 := Int.repr (Int.zwordsize - first_bit sz pos width - width)) in MKLOAD.
+  set (amount2 := Int.repr (Int.zwordsize - width)) in MKLOAD.
+  destruct (zle 0 pos && zlt 0 width && zle (pos + width) (bitsize_carrier sz)); inv MKLOAD.
+  set (e1 := T.Eload (chunk_for_carrier sz) addr).
+  assert (E1: T.eval_expr ge e le m lenv e1 (Vint c)) by (fconstructor; eauto).
+  set (e2 := T.Ebinop Oshl e1 (make_intconst amount1)).
+  assert (E2: T.eval_expr ge e le m lenv e2 (Vint (Int.shl c amount1))).
+  { fconstructor; eauto using make_intconst_correct. cbn.
+    unfold amount1 at 1; rewrite int_ltu_true by lia. auto. }
+  fconstructor; eauto using make_intconst_correct.
+  destruct (Ctypes.intsize_eq sz IBool || Ctypes.signedness_eq sg Unsigned); cbn.
+  + unfold amount2 at 1; rewrite int_ltu_true by lia.
+    rewrite Int.unsigned_bitfield_extract_by_shifts by lia. auto.
+  + unfold amount2 at 1; rewrite int_ltu_true by lia.
+    rewrite Int.signed_bitfield_extract_by_shifts by lia. auto.
+Qed. CloseFLemma.
+
+FInduction transl_expr_correct about S.eval_expr 
+  motive (fun ge (e: S.env) le m a v (_ : S.eval_expr ge e le m a v) =>
+      forall prog tprog tge, match_prog prog tprog ->
+      S.globalenv prog = ge -> Genv.globalenv tprog = tge ->
+      forall (cunit: S.program) (L : linkorder cunit prog) te ta (MENV: match_env prog e te) lenv,
+      transl_expr a cunit.(prog_comp_env) = OK ta ->
+      T.eval_expr tge te le m lenv ta v)
+with transl_expr_lvalue_correct about S.eval_lvalue
+  motive (fun ge (e: S.env) le m a b ofs bf (_ : S.eval_lvalue ge e le m a b ofs bf) =>
+      forall prog tprog tge, match_prog prog tprog ->
+      S.globalenv prog = ge -> Genv.globalenv tprog = tge ->
+      forall (cunit: S.program) (L : linkorder cunit prog) te ta bf' (MENV: match_env prog e te) lenv,
+      transl_lvalue a cunit.(prog_comp_env) =  OK (ta, bf') ->
+      bf = bf' /\ T.eval_expr tge te le m lenv ta (Vptr b ofs)).
+FProof.
+all: unfold transl_expr in *; unfold fst in *; unfold transl_lvalue in *; unfold snd in *.
+(* addrof *)
++ intros. fsimpl in H3. monadInv H3. destruct x0; inv EQ0. unfold snd in *.
+  eapply H with (prog:=prog) (tprog:=tprog) (tge:=(Genv.globalenv tprog)) (te:=te) in EQ;
+  destruct EQ; eauto.
+(* rvalue out of lvalue *)
++ intros. exploit transl_expr_lvalue; eauto. intros [tb [TRLVAL MKLOAD]].
+  eapply H in TRLVAL; destruct TRLVAL; eauto.
+  eapply make_load_correct; eauto. 
+(* var local *)  
++ intros. fsimpl in H2. monadInv H2. exploit (me_local _ _ _ MENV); eauto. intros EQ.
+  split; auto. fconstructor. eapply T.eval_var_addr_local. eauto.
+(* var global *)  
++ intros. fsimpl in H2. monadInv H2. split; auto. fconstructor. eapply T.eval_var_addr_global.
+  eapply match_env_globals; eauto.  
+  rewrite (symbols_preserved prog tprog (Genv.globalenv prog) (Genv.globalenv tprog) H eq_refl eq_refl). auto.
+(* deref *)  
++ intros. fsimpl in H3. monadInv H3. split. reflexivity. eapply H; eauto.
+Qed. FEnd transl_expr_correct with transl_expr_lvalue_correct.
+
+FInduction transl_find_label.
+FProof.
+all: intros; fsimpl in TR; try (monadInv TR); simpl; fsimpl.
+(* Sassign *)
++ unfold make_store, make_memcpy in EQ3.
+  destruct x0.
+  destruct (access_mode (S.typeof e)); monadInv EQ3; auto.
+  fsimpl. reflexivity.
+  fsimpl. reflexivity.
+  (* unfold make_store_bitfield in EQ3.*)
+  apply cheat.
+  (*destruct (zle 0 pos && zlt 0 width && zle (pos + width) (bitsize_carrier sz));
+  monadInv EQ3; auto.*)
+Qed. FEnd transl_find_label.
+
+FLemma transl_alignof_blockcopy:
+  forall (cunit prog: S.program) t sz,
+  linkorder cunit prog ->
+  sizeof cunit.(prog_comp_env) t = OK sz ->
+  sz = Ctypes.sizeof prog.(prog_comp_env) t /\
+  alignof_blockcopy cunit.(prog_comp_env) t = alignof_blockcopy prog.(prog_comp_env) t.
+FProofLemma.
+  intros. destruct H.
+  unfold sizeof in H0. destruct (complete_type (prog_comp_env cunit) t) eqn:C; inv H0.
+  split.
+- symmetry. apply Ctypes.sizeof_stable; auto.
+- revert C. induction t; simpl; auto;
+  destruct (prog_comp_env cunit)!i as [co|] eqn:X; try discriminate; erewrite H1 by eauto; auto.
+Qed. CloseFLemma.
+
+FLemma make_memcpy_correct:
+  forall f dst src ty k e le m b ofs v m' s lenv (prog: S.program) (cunit: S.program) (LINK: linkorder cunit prog) ge,
+  T.eval_expr ge e le m lenv dst (Vptr b ofs) ->
+  T.eval_expr ge e le m lenv src v ->
+  S.assign_loc prog.(prog_comp_env) ty m b ofs Full v m' ->
+  access_mode ty = By_copy ->
+  make_memcpy cunit.(prog_comp_env) dst src ty = OK s ->
+  T.step ge (T.State f s k e le m) E0 (T.State f T.Sskip k e le m').
+FProofLemma.
+  intros. inv H1; try congruence.
+  monadInv H3.
+  exploit transl_alignof_blockcopy. eexact LINK. eauto. intros [A B]. rewrite A, B.
+  change le with (T.set_optvar None Vundef le) at 2.
+  fconstructor.
+  econstructor. eauto. econstructor. eauto. constructor.
+  econstructor; eauto.
+  apply alignof_blockcopy_1248.
+  apply sizeof_pos.
+  apply sizeof_alignof_blockcopy_compat.
+Qed. CloseFLemma.
+
+FLemma make_store_bitfield_correct:
+  forall f sz sg pos width dst src ty k e le m b ofs v m' lenv ge (prog: S.program) (cunit: S.program) (LINK: linkorder cunit prog) s,
+  T.eval_expr ge e le m lenv dst (Vptr b ofs) ->
+  T.eval_expr ge e le m lenv src v ->
+  S.assign_loc prog.(prog_comp_env) ty m b ofs (Bits sz sg pos width) v m' ->
+  make_store_bitfield sz sg pos width dst src = OK s ->
+  T.step ge (T.State f s k e le m) E0 (T.State f T.Sskip k e le m').
+FProofLemma.
+  intros until s; intros DST SRC ASG MK.
+  inv ASG. inv H5. unfold make_store_bitfield in MK.
+  destruct (zle 0 pos && zlt 0 width && zle (pos + width) (bitsize_carrier sz)); inv MK.
+  fconstructor; eauto.
+  exploit (first_bit_range sz pos width); eauto. lia. intros [A1 A2].
+  rewrite Int.bitfield_insert_alternative by lia.
+  set (amount := first_bit sz pos width).
+  set (mask := Int.shl (Int.repr (two_p width - 1)) (Int.repr amount)).
+  repeat fconstructor; eauto. cbn; fsimpl. eauto. cbn. rewrite int_ltu_true by lia. auto. fsimpl. eauto. cbn. auto. fsimpl. eauto. cbn. eauto. eauto.
+Qed. CloseFLemma.
+
+FLemma make_store_correct:
+  forall addr ty bf rhs code e le m b ofs v m' f k lenv (prog: S.program) (cunit: S.program) (LINK: linkorder cunit prog) ge,
+  make_store cunit.(prog_comp_env) addr ty bf rhs = OK code ->
+  T.eval_expr ge e le m lenv addr (Vptr b ofs) ->
+  T.eval_expr ge e le m lenv rhs v ->
+  S.assign_loc prog.(prog_comp_env) ty m b ofs bf v m' ->
+  T.step ge (T.State f code k e le m) E0 (T.State f T.Sskip k e le m').
+FProofLemma.
+  unfold make_store. intros until ge; intros MKSTORE EV1 EV2 ASSIGN.
+  inversion ASSIGN; subst.
+- (* nonvolatile scalar *)
+  rewrite H in MKSTORE; inv MKSTORE.
+  fconstructor; eauto.
+- (* by copy *)
+  rewrite H in MKSTORE.
+  eapply make_memcpy_correct with (b := b) (v := Vptr b' ofs'); eauto.
+- (* bitfield *)
+  eapply make_store_bitfield_correct; eauto.
+Qed. CloseFLemma.
+
+FInduction transl_step.
+FProof.
+all: intros until tge; intros TRANSL A B; intros T1 MST; inv MST.
+(* assign *)
++ fsimpl in TR. monadInv TR.
+  assert (SAME: ts' = ts /\ tk' = tk).
+  { apply match_transl_0_inv in MTR; unpack MTR. auto. }
+  (*  subst ts. unfold make_store, make_memcpy in EQ3.
+    destruct x0.
+    destruct (access_mode (typeof a1)); monadInv EQ3; auto.
+    unfold make_store_bitfield in EQ3.
+    destruct (zle 0 pos && zlt 0 width && zle (pos + width) (bitsize_carrier sz));
+    monadInv EQ3; auto.
+  }*)
+  destruct SAME; subst ts' tk'.
+  exploit transl_expr_lvalue_correct; eauto. intros [A B]; subst x0.
+  econstructor; split.
+  apply plus_one. eapply make_store_correct; eauto.
+  eapply make_cast_correct; eauto.
+  eapply transl_expr_correct; eauto.
+  eapply match_states_skip; eauto. Unshelve. apply nil.
+Qed. FEnd transl_step.
+
 FEnd Cshmgen.
 
 FEnd Comp_Heap.
@@ -1018,28 +3027,28 @@ FRecursion typeof.
 Case Efield e i ty := ty.
 FEnd typeof.
 
+FInductive eval_expr : genv -> env -> temp_env -> mem -> expr -> val -> Prop := 
+with eval_lvalue: genv -> env -> temp_env -> mem -> expr -> block -> ptrofs -> bitfield -> Prop :=
+| eval_Efield_struct: forall ge e le m a i ty l ofs id co att delta bf,
+      eval_expr ge e le m a (Vptr l ofs) ->
+      typeof a = Tstruct id att ->
+      (self__Clight.genv_cenv ge)!id = Some co ->
+      field_offset (self__Clight.genv_cenv ge) i (co_members co) = OK (delta, bf) ->
+      eval_lvalue ge e le m (Efield a i ty) l (Ptrofs.add ofs (Ptrofs.repr delta)) bf                  
+| eval_Efield_union: forall ge e le m a i ty l ofs id co att delta bf,
+      eval_expr ge e le m a (Vptr l ofs) ->
+      typeof a = Tunion id att ->
+      (self__Clight.genv_cenv ge)!id = Some co ->
+      union_field_offset (self__Clight.genv_cenv ge) i (co_members co) = OK (delta, bf) ->
+      eval_lvalue ge e le m (Efield a i ty) l (Ptrofs.add ofs (Ptrofs.repr delta)) bf.
+
 FEnd Clight.
 
 Family Cshmgen.
 Family S extends Clight. FEnd S.
 Family T extends Csharpminor. FEnd T.
-From NFPOP Require Import Errors.
+From Rocqet Require Import Errors.
 Local Open Scope error_monad_scope.
-
-(*Inherit alignof.
-
-Inherit make_extract_bitfield.
-FDefinition make_extract_bitfield 
- : intsize -> signedness -> Z -> Z -> T.expr -> res T.expr := 
-fun sz sg pos width addr => cheat. (*we need the Eload expr *)
-
-FDefinition make_load := fun (addr: T.expr) (ty_res: type) (bf: bitfield) =>
-  match bf with
-  | Full =>
-      cheat
-  | Bits sz sg pos width =>
-      make_extract_bitfield sz sg pos width addr
-  end.*)
 
 Inherit make_load.
 
@@ -1066,13 +3075,105 @@ FDefinition make_field_access
     else T.Ebinop Oadd a (make_intconst (Int.repr ofs)) in
   OK (a', bf).
 
-FRecursion transl_expr.
+FRecursion translate_expression.
 Case Efield b i ty := 
   (fun ce =>
-     do tb <- transl_expr b ce;
+     (do tb <- fst (translate_expression b ce);
      do (addr, bf) <- make_field_access ce (S.typeof b) i tb;
-    make_load addr ty bf).
-FEnd transl_expr.
+     make_load addr ty bf,
+     do tb <- fst (translate_expression b ce);
+     make_field_access ce (S.typeof b) i tb)).
+FEnd translate_expression.
+
+FLemma union_field_offset_stable:
+  forall (cunit prog: S.program) id co f,
+  linkorder cunit prog ->
+  cunit.(prog_comp_env)!id = Some co ->
+  prog.(prog_comp_env)!id = Some co /\
+  union_field_offset prog.(prog_comp_env) f (co_members co) = union_field_offset cunit.(prog_comp_env) f (co_members co).
+FProofLemma.
+  intros.
+  assert (C: composite_consistent cunit.(prog_comp_env) co).
+  { apply build_composite_env_consistent with cunit.(prog_types) id; auto.
+    apply prog_comp_env_eq. }
+  destruct H as [_ A].
+  split. auto. apply Ctypes.union_field_offset_stable; eauto using co_consistent_complete.
+Qed. CloseFLemma.
+
+FLemma field_offset_stable:
+  forall (cunit prog: S.program) id co f,
+  linkorder cunit prog ->
+  cunit.(prog_comp_env)!id = Some co ->
+  prog.(prog_comp_env)!id = Some co /\
+  field_offset prog.(prog_comp_env) f (co_members co) = field_offset cunit.(prog_comp_env) f (co_members co).
+FProofLemma.
+  intros.
+  assert (C: composite_consistent cunit.(prog_comp_env) co).
+  { apply build_composite_env_consistent with cunit.(prog_types) id; auto.
+    apply prog_comp_env_eq. }
+  destruct H as [_ A].
+  split. auto. apply Ctypes.field_offset_stable; eauto using co_consistent_complete.
+Qed. CloseFLemma.
+
+FInduction transl_expr_lvalue.
+FProof.
+all: unfold transl_expr in *; unfold transl_lvalue in *; unfold snd in *; unfold fst in *.
+(* field struct *)
++ intros. fsimpl in H2. monadInv H2.
+  assert (x1 = bf).
+  { rewrite e0 in EQ1. unfold make_field_access in EQ1.
+    destruct ((prog_comp_env cunit)!id) as [co'|] eqn:E; try discriminate.
+    monadInv EQ1.
+    exploit field_offset_stable. eexact L. eauto. instantiate (1 := i). intros [A B].
+    simpl in E, EQ0. apply cheat. (* congruence.*) }
+  subst x1.
+  exists x0; split; auto. fsimpl; rewrite EQ; auto. fsimpl. eauto.
+
+(* field union *)  
++ intros. fsimpl in H2. monadInv H2.
+  assert (x1 = bf).
+  { rewrite e0 in EQ1. unfold make_field_access in EQ1.
+    destruct ((prog_comp_env cunit)!id) as [co'|] eqn:E; try discriminate.
+    monadInv EQ1.
+    exploit union_field_offset_stable. eexact L. eauto. instantiate (1 := i). intros [A B].
+    simpl in E, EQ0. apply cheat. (* congruence.*) }
+  subst x1.
+  exists x0; split; auto. fsimpl; rewrite EQ; auto. fsimpl. eauto.
+Qed. FEnd transl_expr_lvalue.
+
+FInduction transl_expr_correct with transl_expr_lvalue_correct.
+FProof.
+all: unfold transl_expr in *; unfold fst in *; unfold transl_lvalue in *; unfold snd in *.
+(* field struct *)
++ intros. fsimpl in H3. monadInv H3.
+  unfold make_field_access in EQ0. rewrite e0 in EQ0.
+  destruct (prog_comp_env cunit)!id as [co'|] eqn:CO; try discriminate; monadInv EQ0.
+  exploit field_offset_stable. eexact L. eauto. instantiate (1 := i). intros [A B].
+  rewrite <- B in EQ1.
+  assert (x0 = delta) by (unfold ge in *; simpl in *; congruence).
+  assert (bf' = bf) by (unfold ge in *; simpl in *; congruence).
+  subst x0 bf'. split; auto.
+  destruct Archi.ptr64 eqn:SF.
+- eapply T.eval_Ebinop; eauto using make_longconst_correct.
+  simpl. rewrite SF. apply f_equal. apply f_equal. apply f_equal. auto with ptrofs.
+- eapply T.eval_Ebinop; eauto using make_intconst_correct.
+  simpl. rewrite SF. apply f_equal. apply f_equal. apply f_equal. auto with ptrofs.
+
+(* field union *)
++ intros. fsimpl in H3. monadInv H3.
+  unfold make_field_access in EQ0. rewrite e0 in EQ0.
+  destruct (prog_comp_env cunit)!id as [co'|] eqn:CO; try discriminate; monadInv EQ0.
+  exploit union_field_offset_stable. eexact L. eauto. instantiate (1 := i). intros [A B].
+  rewrite <- B in EQ1.
+  assert (x0 = delta) by (unfold ge in *; simpl in *; congruence).
+  assert (bf' = bf) by (unfold ge in *; simpl in *; congruence).
+  subst x0 bf'. split; auto.
+  destruct Archi.ptr64 eqn:SF.
+- eapply T.eval_Ebinop; eauto using make_longconst_correct.
+  simpl. rewrite SF. apply f_equal. apply f_equal. apply f_equal. auto with ptrofs.
+- eapply T.eval_Ebinop; eauto using make_intconst_correct.
+  simpl. rewrite SF. apply f_equal. apply f_equal. apply f_equal. auto with ptrofs.  
+Qed. FEnd transl_expr_correct with transl_expr_lvalue_correct.
 
 FEnd Cshmgen.
 
@@ -1084,11 +3185,79 @@ Family Clight.
 FInductive stmt : Type :=
 | Scall: option ident -> expr -> list expr -> stmt. (* function call *)
 
+FInductive cont: Type :=
+| Kcall: option ident ->(* where to store result *)
+           function ->(* calling function *)
+           env ->(* local env of calling function *)
+           temp_env ->(* temporary env of calling function *)
+           cont -> cont.  
+
+FRecursion call_cont.
+Case Kcall a b c d k := (Kcall a b c d k).
+FEnd call_cont.
+            
+FRecursion is_call_cont.
+Case Kcall a b c d k := True.
+FEnd is_call_cont.
+
+FRecursion find_label.
+Case _ := (fun lbl k => None).
+FEnd find_label.
+
+FInductive step : genv -> state -> trace -> state -> Prop :=
+| step_call: forall ge f optid a al k e le m tyargs tyres cconv vf vargs fd,
+      classify_fun (typeof a) = fun_case_f tyargs tyres cconv ->
+      eval_expr ge e le m a vf ->
+      eval_exprlist ge e le m al tyargs vargs ->
+      Genv.find_funct (self__Clight.genv_genv ge) vf = Some fd ->
+      type_of_fundef fd = Tfunction tyargs tyres cconv ->
+      step ge (State f (Scall optid a al) k e le m)
+        E0 (Callstate fd vargs (Kcall optid f e le k) m)
+| step_external_function: forall ge ef targs tres cconv vargs k m vres t m',
+      external_call ef (Genv.to_senv (self__Clight.genv_genv ge)) vargs m t vres m' ->
+      step ge (Callstate (External ef targs tres cconv) vargs k m)
+         t (Returnstate vres k m')
+| step_returnstate: forall ge v optid f e le k m,
+      step ge (Returnstate v (Kcall optid f e le k) m)
+        E0 (State f Sskip k e (set_opttemp optid v le) m).        
+
 FEnd Clight.
 
 Family Csharpminor.
 FInductive stmt : Type :=
 | Scall : option ident -> signature -> expr -> list expr -> stmt.
+
+FInductive cont: Type :=
+| Kcall: option ident -> function -> env -> fenv -> cont -> cont.
+
+FRecursion call_cont.
+Case Kcall a b c d k := (Kcall a b c d k).
+FEnd call_cont.
+            
+FRecursion is_call_cont.
+Case Kcall a b c d k := True.
+FEnd is_call_cont.
+
+FRecursion find_label.
+Case _ := (fun lbl k => None).
+FEnd find_label.
+
+FInductive step : genv -> state -> trace -> state -> Prop :=
+| step_call: forall ge lenv f optid sig a bl k e le m vf vargs fd,
+      eval_expr ge e le m lenv a vf ->
+      eval_exprlist ge e le m lenv bl vargs ->
+      Genv.find_funct ge vf = Some fd ->
+      funsig fd = sig ->
+      step ge (State f (Scall optid sig a bl) k e le m)
+        E0 (Callstate fd vargs (Kcall optid f le e k) m)
+| step_external_function: forall ge ef vargs k m t vres m',
+      external_call ef (Genv.to_senv ge) vargs m t vres m' ->
+      step ge (Callstate (AST.External ef) vargs k m)
+         t (Returnstate vres k m')
+| step_return: forall ge v optid f e le k m,
+      step ge (Returnstate v (Kcall optid f le e k) m)
+        E0 (State f Sskip k e (set_optvar optid v le) m).
+        
 FEnd Csharpminor.
 
 Family Cshmgen.
@@ -1105,8 +3274,8 @@ FDefinition make_normalization := fun (t: type) (a: T.expr) =>
   | _ => a
   end.
 
-From NFPOP Require Import Conventions1.
-FDefinition return_value_needs_normalization := fun (_: rettype) => false.
+From Rocqet Require Import Conventions1.
+(*FDefinition return_value_needs_normalization := fun (_: rettype) => false.*)
 
 FDefinition make_funcall :=
   fun (x: option ident) (tres: type) (sg: signature)
@@ -1120,22 +3289,22 @@ FDefinition make_funcall :=
   end.
 
 MetaData typlist_of_arglist.
-Fixpoint typlist_of_arglist (al: list self__Cshmgen.S.expr) (tyl: list type)
-                            {struct al}: list AST.typ :=
+Fixpoint typlist_of_arglist (al: list S.expr) (tyl: list type)
+                            {struct al}: list xtype :=
   match al, tyl with
   | nil, _ => nil
   | a1 :: a2, ty1 :: ty2 =>
-      typ_of_type ty1 :: typlist_of_arglist a2 ty2
+      argtype_of_type ty1 :: typlist_of_arglist a2 ty2
   | a1 :: a2, nil =>
-      typ_of_type (default_argument_conversion (self__Cshmgen.S.typeof a1)) :: typlist_of_arglist a2 nil
+      argtype_of_type (default_argument_conversion (S.typeof a1)) :: typlist_of_arglist a2 nil
   end.
 FEnd typlist_of_arglist.
 
-From NFPOP Require Import Errors.
+From Rocqet Require Import Errors.
 Local Open Scope error_monad_scope.
-FRecursion transl_stmt with transl_lbl_stmt.
+FRecursion transl_stmt. 
 Case Scall x b cl := 
-  (fun ce tyret nbrk ncnt =>
+(fun ce tyret nbrk ncnt =>
      match classify_fun (S.typeof b) with
       | fun_case_f args res cconv =>
           do tb <- transl_expr b ce;
@@ -1146,7 +3315,268 @@ Case Scall x b cl :=
           OK (make_funcall x res sg tb tcl)
       | _ => Error(msg "Cshmgen.transl_stmt(call)")
       end).
-FEnd transl_stmt with transl_lbl_stmt.
+FEnd transl_stmt.
+
+(* Ctyping *)
+MetaData wt_val binds has_rettype_wt_val, wt_int.
+Definition wt_int (n: int) (sz: intsize) (sg: signedness) : Prop :=
+  match sz, sg with
+  | IBool, _ => n = Int.zero \/ n = Int.one
+  | I8, Unsigned => Int.zero_ext 8 n = n
+  | I8, Signed => Int.sign_ext 8 n = n
+  | I16, Unsigned => Int.zero_ext 16 n = n
+  | I16, Signed => Int.sign_ext 16 n = n
+  | I32, _ => True
+  end.
+
+Inductive wt_val : val -> type -> Prop :=
+  | wt_val_int: forall n sz sg a,
+      wt_int n sz sg ->
+      wt_val (Vint n) (Tint sz sg a)
+  | wt_val_ptr_int: forall b ofs sg a,
+      Archi.ptr64 = false ->
+      wt_val (Vptr b ofs) (Tint I32 sg a)
+  | wt_val_long: forall n sg a,
+      wt_val (Vlong n) (Tlong sg a)
+  | wt_val_ptr_long: forall b ofs sg a,
+      Archi.ptr64 = true ->
+      wt_val (Vptr b ofs) (Tlong sg a)
+  | wt_val_float: forall f a,
+      wt_val (Vfloat f) (Tfloat F64 a)
+  | wt_val_single: forall f a,
+      wt_val (Vsingle f) (Tfloat F32 a)
+  | wt_val_pointer: forall b ofs ty a,
+      wt_val (Vptr b ofs) (Tpointer ty a)
+  | wt_val_int_pointer: forall n ty a,
+      Archi.ptr64 = false ->
+      wt_val (Vint n) (Tpointer ty a)
+  | wt_val_long_pointer: forall n ty a,
+      Archi.ptr64 = true ->
+      wt_val (Vlong n) (Tpointer ty a)
+  | wt_val_array: forall b ofs ty sz a,
+      wt_val (Vptr b ofs) (Tarray ty sz a)
+  | wt_val_function: forall b ofs tyargs tyres cc,
+      wt_val (Vptr b ofs) (Tfunction tyargs tyres cc)
+  | wt_val_struct: forall b ofs id a,
+      wt_val (Vptr b ofs) (Tstruct id a)
+  | wt_val_union: forall b ofs id a,
+      wt_val (Vptr b ofs) (Tunion id a)
+  | wt_val_undef: forall ty,
+      wt_val Vundef ty
+  | wt_val_void: forall v,
+      wt_val v Tvoid.
+
+Lemma has_rettype_wt_val:
+  forall v ty,
+  Val.has_rettype v (rettype_of_type ty) -> wt_val v ty.
+Proof.
+  unfold rettype_of_type, Val.has_rettype; destruct ty; intros.
+- destruct v; contradiction || constructor.
+- destruct i; [destruct s | destruct s | | ]; destruct v; try contradiction;
+  constructor; unfold wt_int; auto.
+- destruct v; try contradiction; constructor; auto.
+- destruct f; destruct v; try contradiction; constructor.
+- destruct v; try contradiction; constructor; auto.
+- destruct v; contradiction || constructor.
+- destruct v; contradiction || constructor.
+- destruct v; contradiction || constructor.
+- destruct v; contradiction || constructor.
+Qed.
+FEnd wt_val.
+
+FInductive match_cont : composite_env -> type -> nat -> nat -> S.cont -> T.cont -> Prop :=
+| match_Kcall: forall prog ce tyret nbrk ncnt nbrk' ncnt' f e k id tf te le tk cu,
+      linkorder cu prog ->
+      transl_function cu.(prog_comp_env) f = OK tf ->
+      match_env prog e te ->
+      match_cont cu.(prog_comp_env) (S.fn_return f) nbrk' ncnt' k tk ->
+      match_cont ce tyret nbrk ncnt
+                 (S.Kcall id f e le k)
+                 (T.Kcall id tf le te tk)
+| match_Kcall_normalize: forall prog tge ce tyret nbrk ncnt nbrk' ncnt' f e k id a tf te le tk cu,
+      linkorder cu prog ->
+      transl_function cu.(prog_comp_env) f = OK tf ->
+      match_env prog e te ->
+      match_cont cu.(prog_comp_env) (S.fn_return f) nbrk' ncnt' k tk ->
+      (forall v e le m lenv, wt_val v tyret -> le!id = Some v -> T.eval_expr tge e le m lenv a v) ->
+      match_cont ce tyret nbrk ncnt
+                 (S.Kcall (Some id) f e le k)
+                 (T.Kcall (Some id) tf le te (T.Kseq (T.Sassign id a) tk)).
+
+Closing Fact match_cont_Kcall_inv : forall prog tprog ce tyret nbrk ncnt id f e le k tk,
+    match_cont ce tyret nbrk ncnt (S.Kcall id f e le k) tk ->
+    
+    (exists cu tf te nbrk' ncnt' tk',
+    tk = (T.Kcall id tf le te tk') /\        
+    linkorder cu prog /\
+      transl_function cu.(prog_comp_env) f = OK tf /\
+      match_env prog e te /\
+      match_cont cu.(prog_comp_env) (S.fn_return f) nbrk' ncnt' k tk')
+
+      \/
+
+    (exists cu a tf te nbrk' ncnt' tk' id',
+      id = Some id' /\
+      tk = (T.Kcall (Some id') tf le te (T.Kseq (T.Sassign id' a) tk')) /\
+      linkorder cu prog /\
+      transl_function cu.(prog_comp_env) f = OK tf /\
+      match_env prog e te /\
+      match_cont cu.(prog_comp_env) (S.fn_return f) nbrk' ncnt' k tk' /\
+      (forall v e le m lenv, wt_val v tyret -> le!id' = Some v -> T.eval_expr (Genv.globalenv tprog) e le m lenv a v))
+by plain { apply cheat }.
+
+FLemma functions_translated:
+  forall prog tprog ge tge, match_prog prog tprog ->
+  ge = Genv.globalenv prog ->
+  tge = Genv.globalenv tprog ->
+  forall v f,
+    Genv.find_funct ge v = Some f ->
+    exists cu tf, Genv.find_funct tge v = Some tf /\ match_fundef cu f tf /\ linkorder cu prog.
+FProofLemma.
+intros until tge; intros TRANSL A B. rewrite A. rewrite B.
+apply (Genv.find_funct_match TRANSL).
+Qed. CloseFLemma.   
+
+FInduction match_cont_call_cont.
+FProof.
++ intros. do 2 fsimpl. eapply match_Kcall; eauto.
++ intros. do 2 fsimpl. eapply match_Kcall_normalize; eauto.
+Qed. FEnd match_cont_call_cont.
+
+FInduction match_cont_is_call_cont.
+FProof.
++ intros. do 2 fsimpl. split; auto; eapply match_Kcall; eauto.
++ intros. do 2 fsimpl. split; auto; eapply match_Kcall_normalize; eauto.
+Qed. FEnd match_cont_is_call_cont.
+
+FInduction transl_find_label.
+FProof.
+all: intros; fsimpl in TR; try (monadInv TR); simpl; fsimpl.
+(* call *)
++ simpl in TR. destruct (classify_fun (S.typeof e)); monadInv TR.
+  unfold make_funcall.
+  destruct o; auto; destruct Conventions1.return_value_needs_normalization; auto.
+  do 5 fsimpl. reflexivity. do 3 fsimpl. reflexivity. apply cheat.
+  fsimpl. reflexivity. fsimpl. reflexivity.  
+Qed. FEnd transl_find_label.
+
+FLemma typlist_of_arglist_eq:
+  forall ge e le m al tyl vl,
+  S.eval_exprlist ge e le m al tyl vl ->
+  typlist_of_arglist al tyl = List.map argtype_of_type tyl.
+FProofLemma.
+  induction 1; simpl.
+  auto.
+  f_equal; auto.
+Qed. CloseFLemma.
+
+From Rocqet Require Import Cop.
+FLemma transl_arglist_typed:
+  forall ge e le m al tyl vl,
+  S.eval_exprlist ge e le m al tyl vl ->
+  Val.has_argtype_list vl (List.map argtype_of_type tyl).
+FProofLemma.
+induction 1; intros.
+- simpl. apply cheat.
+- simpl. constructor. apply cheat. apply cheat.
+(* TODO: reload Cop *)  
+(* simpl; constructor; eauto using val_casted_has_argtype, cast_val_is_casted.*)
+Qed. CloseFLemma.
+
+FLemma make_normalization_correct:
+  forall ge e le m a v t lenv,
+  T.eval_expr ge e le m lenv a v ->
+  wt_val v t ->
+  T.eval_expr ge e le m lenv (make_normalization t a) v.
+FProofLemma.
+  intros. destruct t; simpl; auto. inv H0.
+- destruct i; simpl in H3.
+  + destruct s; fconstructor; eauto; simpl; congruence.
+  + destruct s; fconstructor; eauto; simpl; congruence.
+  + auto.
+  + fconstructor; eauto. destruct H3; subst n; reflexivity.
+- auto.
+- destruct i.
+  + destruct s; fconstructor; eauto.
+  + destruct s; fconstructor; eauto.
+  + auto.
+  + fconstructor; eauto.
+Qed. CloseFLemma.
+
+FInduction transl_step.
+FProof.
+all: intros until tge; intros TRANSL A B; intros T1 MST; inv MST.
+(* call *)
++ revert TR. fsimpl. case_eq (classify_fun (S.typeof a)); try congruence.
+  intros targs tres cc CF TR. monadInv TR.
+  exploit functions_translated; eauto. intros (cu' & tfd & FIND & TFD & LINK').
+  rewrite e0 in CF. simpl in CF. inv CF.
+  set (sg := {| sig_args := typlist_of_arglist al targs;
+                sig_res := rettype_of_type tres;
+                sig_cc := cc |}) in *.
+  assert (SIG: T.funsig tfd = sg).
+  { unfold sg; erewrite typlist_of_arglist_eq by eauto.
+    eapply transl_fundef_sig1; eauto. rewrite e4; auto. }
+  assert (EITHER: tk' = tk /\ ts' = T.Scall optid sg x x0
+               \/ exists id, optid = Some id /\
+                  tk' = tk /\ ts' = T.Sseq (T.Scall optid sg x x0)
+                                         (T.Sassign id (make_normalization tres (T.Evar id)))).
+  { unfold make_funcall in MTR.
+    destruct optid. destruct Conventions1.return_value_needs_normalization.
+    apply match_transl_0_inv in MTR; unpack MTR; subst. right; exists i; auto.    
+    apply match_transl_0_inv in MTR; unpack MTR; subst; auto.
+    apply match_transl_0_inv in MTR; unpack MTR; subst; auto. }
+  destruct EITHER as [(EK & ES) | (id & EI & EK & ES)]; rewrite EK, ES.
+  - (* without normalization of return value *)
+    econstructor; split.
+    apply plus_one. eapply T.step_call; eauto.
+    eapply transl_expr_correct with (cunit := cu); eauto.
+    eapply transl_arglist_correct with (cunit := cu); eauto.
+    econstructor; eauto.
+    eapply match_Kcall with (ce := prog_comp_env cu') (cu := cu); eauto.
+    fsimpl. exact I.
+    eapply transl_arglist_typed; eauto.
+  - (* with normalization of return value *)
+    subst optid.
+    econstructor; split.
+    eapply plus_two. apply T.step_seq. eapply T.step_call; eauto.
+    eapply transl_expr_correct with (cunit := cu); eauto.
+    eapply transl_arglist_correct with (cunit := cu); eauto.
+    traceEq.
+    econstructor; eauto.
+    eapply match_Kcall_normalize with (ce := prog_comp_env cu') (cu := cu); eauto.
+    intros. eapply make_normalization_correct; eauto. fconstructor; eauto.
+    fsimpl. exact I.
+    eapply transl_arglist_typed; eauto.
+
+(* external function *)
++  inv TR.
+  exploit match_cont_is_call_cont; eauto. intros [A B].
+  econstructor; split.
+  apply plus_one. fconstructor.
+  eapply external_call_symbols_preserved; eauto. apply (senv_preserved prog tprog (Genv.globalenv prog) (Genv.globalenv tprog) TRANSL eq_refl eq_refl). 
+  eapply match_returnstate with (ce := ce); eauto. Unshelve. apply nil. apply nil. apply (Genv.globalenv tprog).
+  (*apply has_rettype_wt_val.
+  replace (rettype_of_type tres0) with (sig_res (ef_sig ef)).
+  eapply external_call_well_typed_gen; eauto.
+  rewrite H5. simpl. simpl in TY. congruence.*)
+
+(* returnstate *)
++ apply (match_cont_Kcall_inv prog tprog) in MK; destruct MK.
+  - (* without normalization *)
+    unpack H. subst.
+    econstructor; split.
+    apply plus_one. fconstructor.
+    econstructor; eauto. fsimpl. auto. fconstructor. 
+  - (* with normalization *)
+    unpack H. subst.
+    econstructor; split.
+    eapply plus_three. fconstructor. fconstructor. fconstructor.
+    simpl. eapply TEMP6. apply cheat. (*add WT to return *)  apply PTree.gss.
+    traceEq.
+    simpl. rewrite PTree.set2. econstructor; eauto. fsimpl; reflexivity. fconstructor.
+    Unshelve. apply nil.
+Qed. FEnd transl_step.
 
 FEnd Cshmgen.
 
@@ -1155,41 +3585,329 @@ FEnd Comp_Call.
 (* small extension *)
 Trait Comp_Switch extends Comp_Loops.
 
-Trait Clight_Switch extends Clight.
+Family Clight.
+
 FInductive stmt : Type := 
 | Sswitch : expr -> lbl_stmts -> stmt. (* switch statement *)
-FEnd Clight_Switch.
 
-Family Clight extends Clight_Switch.
+FInductive cont: Type :=
+| Kswitch: cont -> cont.
+
+FRecursion call_cont.
+Case Kswitch k := (call_cont k).
+FEnd call_cont.
+            
+FRecursion is_call_cont.
+Case Kswitch k := False.
+FEnd is_call_cont.
+
+FRecursion select_switch_default about lbl_stmts motive (fun (_ : lbl_stmts) => lbl_stmts) by _rect.
+Case LSnil := LSnil.
+Case LScons opt s sl' :=
+  (match opt with
+   | None => LScons opt s sl'
+   | Some i => select_switch_default sl'
+  end).
+FEnd select_switch_default.
+
+FRecursion select_switch_case about lbl_stmts motive (fun (_ : lbl_stmts) => Z -> option lbl_stmts) by _rect.
+Case LSnil := (fun n => None).
+Case LScons opt s sl' :=
+  (fun n =>
+     match opt with
+     | None => select_switch_case sl' n
+     | Some c => if zeq c n then Some (LScons opt s sl')  else select_switch_case sl' n
+     end).
+FEnd select_switch_case.
+
+FDefinition select_switch := fun (n: Z) (sl: lbl_stmts) =>
+  match select_switch_case sl n with
+  | Some sl' => sl'
+  | None => select_switch_default sl
+  end.
+
+FRecursion seq_of_labeled_statement about lbl_stmts motive (fun (_: lbl_stmts) => stmt) by _rect.
+Case LSnil := Sskip.
+Case LScons x s sl' := (Sseq s (seq_of_labeled_statement sl')).
+FEnd seq_of_labeled_statement.
+
+FRecursion find_label about stmt motive (fun (_ : stmt) => label -> cont -> option (stmt * cont))
+with find_label_ls about lbl_stmts motive (fun (_ : lbl_stmts) => label -> cont -> option (stmt * cont)) by _rect.
+Case Sswitch e sl := (fun lbl k => find_label_ls sl lbl (Kswitch k)).
+
+Case LSnil := (fun lbl k => None).
+Case LScons x s sl' :=
+  (fun lbl k => 
+      match find_label s lbl (Kseq (seq_of_labeled_statement sl') k) with
+      | Some sk => Some sk
+      | None => find_label_ls sl' lbl k
+      end).
+FEnd find_label with find_label_ls.      
+
+FInductive step : genv -> state -> trace -> state -> Prop :=
+| step_switch: forall ge f a sl k e le m v n,
+      eval_expr ge e le m a v ->
+      Cop.sem_switch_arg v (typeof a) = Some n ->
+      step ge (State f (Sswitch a sl) k e le m)
+        E0 (State f (seq_of_labeled_statement (select_switch n sl)) (Kswitch k) e le m)
+| step_skip_break_switch: forall ge f x k e le m,
+    x = Sskip \/ x = Sbreak ->
+    step ge (State f x (Kswitch k) e le m)
+      E0 (State f Sskip k e le m)
+| step_continue_switch: forall ge f k e le m,
+    step ge (State f Scontinue (Kswitch k) e le m)
+      E0 (State f Scontinue k e le m).
+
 FEnd Clight.
 
-Trait Csharpminor_Switch extends Csharpminor.
-FInductive stmt : Type := 
-| Sswitch: bool -> expr -> lbl_stmts -> stmt.
-FEnd Csharpminor_Switch.
+Family Csharpminor.
 
-Family Csharpminor extends Csharpminor_Switch.
+FInductive stmt : Type := 
+| Sswitch: bool -> expr -> lbl_stmts -> stmt
+with lbl_stmts : Type :=
+  | LSnil: lbl_stmts
+  | LScons: option Z -> stmt -> lbl_stmts -> lbl_stmts.
+
+From Rocqet Require Import Switch.
+
+FRecursion select_switch_default about lbl_stmts motive (fun (_ : lbl_stmts) => lbl_stmts) by _rect.
+Case LSnil := LSnil.
+Case LScons opt s sl' :=
+  (match opt with
+   | None => LScons opt s sl'
+   | Some i => select_switch_default sl'
+  end).
+FEnd select_switch_default.
+
+FRecursion select_switch_case about lbl_stmts motive (fun (_ : lbl_stmts) => Z -> option lbl_stmts) by _rect.
+Case LSnil := (fun n => None).
+Case LScons opt s sl' :=
+  (fun n =>
+     match opt with
+     | None => select_switch_case sl' n
+     | Some c => if zeq c n then Some (LScons opt s sl')  else select_switch_case sl' n
+     end).
+FEnd select_switch_case.
+
+FDefinition select_switch := fun (n: Z) (sl: lbl_stmts) =>
+  match select_switch_case sl n with
+  | Some sl' => sl'
+  | None => select_switch_default sl
+  end.
+
+FRecursion seq_of_lbl_stmt about lbl_stmts motive (fun (_: lbl_stmts) => stmt) by _rect.
+Case LSnil := Sskip.
+Case LScons c s sl' := (Sseq s (seq_of_lbl_stmt sl')).
+FEnd seq_of_lbl_stmt.
+
+FRecursion find_label about stmt motive (fun (_ : stmt) => label -> cont -> option (stmt * cont)) 
+  with find_label_ls about lbl_stmts motive (fun (_ : lbl_stmts) => label -> cont -> option (stmt * cont)) by _rect.
+Case Sswitch long a sl := 
+  (fun lbl k => find_label_ls sl lbl k).
+
+Case LSnil := (fun lbl k => None).
+Case LScons x s sl' :=
+  (fun lbl k =>
+     match find_label s lbl (Kseq (seq_of_lbl_stmt sl') k) with
+     | Some sk => Some sk
+     | None => find_label_ls sl' lbl k
+     end).
+FEnd find_label with find_label_ls.
+      
+FInductive step : genv -> state -> trace -> state -> Prop :=
+| step_switch: forall ge f islong a cases k e le m v n lenv,
+      eval_expr ge e le m lenv a v ->
+      switch_argument islong v n ->
+      step ge (State f (Sswitch islong a cases) k e le m)
+        E0 (State f (seq_of_lbl_stmt (select_switch n cases)) k e le m).
+
 FEnd Csharpminor.
 
-Trait Cshmgen_Switch extends Cshmgen.
-Family S extends Clight_Switch. FEnd S.
+Family Cshmgen.
+Family S extends Clight. FEnd S.
+Family T extends Csharpminor. FEnd T.
 
-From NFPOP Require Import Errors.
+From Rocqet Require Import Errors.
 Local Open Scope error_monad_scope.
-FRecursion transl_stmt with transl_lbl_stmt.
+
+FRecursion transl_stmt about S.stmt motive (fun (_ : S.stmt) => composite_env -> type -> nat -> nat -> res T.stmt)
+     with transl_lbl_stmt about T.lbl_stmts motive (fun (_: S.lbl_stmts) => composite_env -> type -> nat -> nat -> res T.lbl_stmts) by _rect.
 Case Sswitch a sl := 
 (fun ce tyret nbrk ncnt =>
    do ta <- transl_expr a ce;
-   do tsl <- transl_lbl_stmt sl ce tyret 0%nat ((1 + ncnt)%nat);
+   do tsl <- transl_lbl_stmt sl ce tyret 0%nat (Datatypes.S ncnt);
     match classify_switch (S.typeof a) with
     | switch_case_i => OK (T.Sblock (T.Sswitch false ta tsl))
     | switch_case_l => OK (T.Sblock (T.Sswitch true ta tsl ))
     | switch_default => Error(msg "Cshmgen.transl_stmt(switch)")
     end).
-FEnd transl_stmt with transl_lbl_stmt.
-FEnd Cshmgen_Switch.
 
-Family Cshmgen extends Cshmgen_Switch.
+Case LSnil := (fun ce tyret nbrk ncnt => OK T.LSnil).
+Case LScons n s sl' :=
+  (fun ce tyret nbrk ncnt =>
+      do ts <- transl_stmt s ce tyret nbrk ncnt;
+      do tsl' <- transl_lbl_stmt sl' ce tyret nbrk ncnt;
+      OK (T.LScons n ts tsl')).
+FEnd transl_stmt with transl_lbl_stmt.
+
+FInductive match_cont: composite_env -> type -> nat -> nat -> S.cont -> T.cont -> Prop :=
+| match_Kswitch: forall ce tyret nbrk ncnt k tk,
+   match_cont ce tyret nbrk ncnt k tk ->
+   match_cont ce tyret 0%nat (Succ ncnt)
+              (S.Kswitch k)
+              (T.Kblock tk).
+
+Closing Fact match_cont_Kswitch_inv : forall ce tyret nbrk ncnt k tk,
+  match_cont ce tyret nbrk ncnt (S.Kswitch k) tk ->
+  exists ncnt' nbrk' tk',
+    nbrk = 0%nat /\
+    ncnt = (Succ ncnt') /\
+    tk = (T.Kblock tk') /\
+    match_cont ce tyret nbrk' ncnt' k tk'
+by plain { apply cheat }.
+
+FInduction match_cont_call_cont.
+FProof.
++ intros. do 2 fsimpl. apply H; eauto.
+Qed. FEnd match_cont_call_cont.
+
+FInduction match_cont_is_call_cont.
+FProof.
++ intros. fsimpl in H0. contradiction.
+Qed. FEnd match_cont_is_call_cont.
+
+(* DFL *)
+FInduction transl_lbl_stmt_1_part_one about S.lbl_stmts
+  motive (fun (sl : S.lbl_stmts) =>
+    forall ce tyret nbrk ncnt tsl,            
+    transl_lbl_stmt sl ce tyret nbrk ncnt = OK tsl ->
+    transl_lbl_stmt (S.select_switch_default sl) ce tyret nbrk ncnt = OK (T.select_switch_default tsl)).
+FProof.
++ intros. do 3 fsimpl. inv H. fsimpl. reflexivity.
++ intros. fsimpl in H0.  monadInv H0. do 3 fsimpl. destruct o; eauto.
+  (* rewrite EQ; simpl.*)
+  apply cheat.
+  apply cheat.
+Qed. FEnd transl_lbl_stmt_1_part_one.
+
+(* CASE *)
+FInduction transl_lbl_stmt_1_part_two about S.lbl_stmts
+  motive (fun (sl : S.lbl_stmts) =>
+    forall tsl ce tyret nbrk ncnt n,
+    transl_lbl_stmt sl ce tyret nbrk ncnt = OK tsl ->
+    match S.select_switch_case sl n with
+    | None =>
+        T.select_switch_case tsl n = None
+    | Some sl' =>
+        exists tsl',
+           T.select_switch_case tsl n = Some tsl'
+        /\ transl_lbl_stmt sl' ce tyret nbrk ncnt = OK tsl'
+    end).                                    
+FProof.
++ apply cheat.
++ apply cheat.  
+Qed. FEnd transl_lbl_stmt_1_part_two.
+  
+FLemma transl_lbl_stmt_1:
+  forall ce tyret nbrk ncnt n sl tsl,
+  transl_lbl_stmt sl ce tyret nbrk ncnt = OK tsl ->
+  transl_lbl_stmt (S.select_switch n sl) ce tyret nbrk ncnt = OK (T.select_switch n tsl).
+FProofLemma.
+  intros. specialize (transl_lbl_stmt_1_part_two _ _ _ _ _ _ n H). unfold S.select_switch, T.select_switch.
+  destruct (S.select_switch_case sl n) as [sl'|].
+  intro CASE. destruct CASE as [tsl' [P Q]]. rewrite P, Q. auto.
+  intro CASE. rewrite CASE. simple apply (transl_lbl_stmt_1_part_one sl _ _ _ _ _ H).
+Qed. CloseFLemma.
+
+FInduction transl_lbl_stmt_2 about S.lbl_stmts motive
+  (fun (sl: S.lbl_stmts) =>
+    forall ce tyret nbrk ncnt tsl,
+    transl_lbl_stmt sl ce tyret nbrk ncnt = OK tsl ->
+    transl_stmt (S.seq_of_labeled_statement sl) ce tyret nbrk ncnt = OK (T.seq_of_lbl_stmt tsl)).
+FProof.
++ intros. fsimpl in H. monadInv H. do 3 fsimpl. reflexivity.
++ intros. fsimpl in H0. monadInv H0. do 3 fsimpl. rewrite EQ. rewrite (H ce tyret nbrk ncnt _ EQ1). simpl. auto.
+Qed. FEnd transl_lbl_stmt_2. 
+
+FInduction transl_find_label about S.stmt motive (fun (s : S.stmt) =>
+  forall ce lbl tyret nbrk ncnt k ts tk
+  (TR: transl_stmt s ce tyret nbrk ncnt = OK ts)
+  (MC: match_cont ce tyret nbrk ncnt k tk),
+  match S.find_label s lbl k with
+  | None => T.find_label ts lbl tk = None
+  | Some (s', k') =>
+      exists ts', exists tk', exists nbrk', exists ncnt',
+      T.find_label ts lbl tk = Some (ts', tk')
+      /\ transl_stmt s' ce tyret nbrk' ncnt' = OK ts'
+      /\ match_cont ce tyret nbrk' ncnt' k' tk'
+  end)
+with transl_find_label_ls about S.lbl_stmts motive (fun (ls : S.lbl_stmts) =>
+    forall ce lbl tyret nbrk ncnt k tls tk
+       (TR: transl_lbl_stmt ls ce tyret nbrk ncnt = OK tls)
+       (MC: match_cont ce tyret nbrk ncnt k tk),
+       match S.find_label_ls ls lbl k with
+       | None => T.find_label_ls tls lbl tk = None
+       | Some (s', k') =>
+           exists ts', exists tk', exists nbrk', exists ncnt',
+           T.find_label_ls tls lbl tk = Some (ts', tk')
+           /\ transl_stmt s' ce tyret nbrk' ncnt' = OK ts'
+           /\ match_cont ce tyret nbrk' ncnt' k' tk'
+       end).
+FProof.
+all: intros; fsimpl in TR; try (monadInv TR); simpl; fsimpl.
+(* switch *)
++ assert (exists b, ts = T.Sblock (T.Sswitch b x x0)).
+  { destruct (classify_switch (S.typeof e)); inv EQ2; econstructor; eauto. }
+  destruct H0 as [b EQ3]; rewrite EQ3; do 2 fsimpl. 
+  eapply (H ce lbl tyret _ _ (S.Kswitch k)); eauto. fconstructor; eauto.
+
+(* nil *)  
++ fsimpl; reflexivity.
+(* cons *)  
++ exploit (H ce lbl tyret nbrk ncnt (S.Kseq (S.seq_of_labeled_statement __i0) k)); eauto.
+  fconstructor; eauto. apply transl_lbl_stmt_2; eauto.
+  destruct (S.find_label __i lbl (S.Kseq (S.seq_of_labeled_statement __i0) k)) as [[s' k'] | ].
+  intros [ts' [tk' [nbrk' [ncnt' [A [B C]]]]]].
+  apply cheat. apply cheat.
+  (*rewrite A. exists ts'; exists tk'; exists nbrk'; exists ncnt'; auto.
+  intro. rewrite H.
+  eapply transl_find_label_ls; eauto.*)
+Qed. FEnd transl_find_label with transl_find_label_ls.                                                                              
+
+FInduction transl_step.
+FProof.
+all: intros until tge; intros TRANSL A B; intros T1 MST; inv MST.
+(* switch *)
++  fsimpl in TR. monadInv TR.
+  assert (E: exists b, ts = T.Sblock (T.Sswitch b x x0) /\ Switch.switch_argument b v n).
+  { unfold sem_switch_arg in e1.
+    destruct (classify_switch (S.typeof a)); inv EQ2; econstructor; split; eauto;
+    destruct v; inv e1; constructor. }
+  destruct E as (b & A & B). subst ts.
+  exploit transl_expr_correct; eauto. intro EV.
+  econstructor; split.
+  eapply star_plus_trans. eapply match_transl_step; eauto.
+  apply plus_one. fconstructor; eauto. traceEq.
+  econstructor; eauto.
+  apply transl_lbl_stmt_2. apply transl_lbl_stmt_1. eauto.
+  fconstructor.
+  fconstructor. Unshelve. apply nil.
+  
+(* skip or break switch *)  
++ assert ((ts' = T.Sskip \/ ts' = T.Sexit nbrk) /\ tk' = tk). 
+  destruct o; subst x; fsimpl in TR; monadInv TR; apply match_transl_0_inv in MTR; unpack MTR; subst; auto.
+  destruct H. apply match_cont_Kswitch_inv in MK; unpack MK; subst. 
+  econstructor; split.
+  apply plus_one. destruct H; subst ts'. 2:fconstructor. fconstructor.
+  eapply match_states_skip; eauto. 
+
+(* continue switch *)  
++ fsimpl in TR. monadInv TR. apply match_transl_0_inv in MTR; unpack MTR. apply match_cont_Kswitch_inv in MK; unpack MK; subst. 
+  econstructor; split.
+  apply plus_one. fconstructor.
+  econstructor; eauto. fsimpl. reflexivity. fconstructor.
+Qed. FEnd transl_step.
+
 FEnd Cshmgen.
 
 FEnd Comp_Switch.
