casestudies/compcert/lib/Cop.v
@@ -1642,13 +1642,13 @@ Qed.
 (** Moreover, casted values belong to the machine argument type corresponding
     to the C type. *)
 
-(*Lemma val_casted_has_argtype:
+Lemma val_casted_has_argtype:
   forall v ty, val_casted v ty -> Val.has_argtype v (argtype_of_type ty).
 Proof.
   destruct 1; simpl; rewrite ? H; auto.
 - destruct sz; [destruct si | destruct si | | ]; simpl in *; auto.
   destruct (Int.eq n Int.zero); auto.
-Qed.*)
+Qed.
 
 (** Likewise, casted values belong to the machine type corresponding to the
     C type. *)
